\subsection{Main Theorem Proof}
For concise of the proof, we introduce some conventional operators as follows.
\begin{defn}[Subtrace]
  Subtrace: $[ : ] : \mathcal{{T} \to \eventset \to \eventset \to \mathcal{T}}$ 
  \[
    \trace[\event_1 : \event_2] \triangleq
    \left\{
    \begin{array}{ll} 
    \trace'[\event_1: \event_2]             & \trace = \event :: \trace' \land \event \eventneq \event_1 \\
    \event_1 :: \trace'[:\event_2]  & \trace = \event :: \trace' \land \event \eventeq \event_1 \\
    {[]} & \trace = [] \\
    \end{array}
    \right.
  \]
  For any trace $\trace$ and two events $\event_1, \event_2 \in \eventset$,
  $\trace[\event_1 : \event_2]$ takes the subtrace of $\trace$ starting with $\event_1$ and ending with $\event_2$ including $\event_1$ and $\event_2$.
  \\
  We use $\trace[:\event_2] $ as the shorthand of subtrace starting from head and ending with $\event_2$, and similary for $\trace[\event_1:]$.
  \[
    \trace[:\event] \triangleq
    \left\{
    \begin{array}{ll} 
   \event' :: \trace'[: \event]             & \trace = \event' :: \trace' \land \event' \eventneq \event \\
    \event'  & \trace = \event' :: \trace' \land \event' \eventeq \event \\
    {[]}  & \trace = [] 
    \end{array}
    \right.
  % \]
  % \[
    \quad
    \trace[\event: ] \triangleq
    \left\{
    \begin{array}{ll} 
    \trace'[\event: ]     & \trace =  \event' :: \trace' \land \event \eventneq \event' \\
    \event' :: \trace'  & \trace = \event' :: \trace' \land \event \eventeq \event' \\
    {[ ] } & \trace = []
    \end{array}
    \right.
  \]
\end{defn}
%
Program Entry Point: $\entry_c : \mbox{Command} \to \mathbb{N}$ 
\[
  \entry_c \triangleq 
\left\{
  \begin{array}{ll} 
     l       
    & c = [\eskip]{}^l
    \\ 
    l    & c = [\assign{x}{\expr_1}]{}^l
    \\ 
    l      
    & c = \clabel{\assign{x}{\query(\qexpr_1)}}{}^l
    \\
   l
    & c_1 = \eif([b]{}^l, c_t, c_f)
    \\ 
    l         
    & c = \ewhile [b]^l \edo c'
    \\ 
    \entry_{c1}
    & c = c1;c2
  \end{array}
  \right.
\]
%
\begin{thm}[$\eventdep$ implies $\flowsto$]
\label{thm:flowsto_event_soundness}
For every $D \in \dbdom , c \in \cdom, \trace \in \mathcal{T} \st \forall \event_1, \event_2 \in \eventset \st
\event_1, \event_2 \in \eventset^{\asn}$, 
if $\exists \trace' \in \mathcal{T} \st \trace = [\event_1] \tracecat \trace' \tracecat [\event_2]$ and 
$\eventdep(\event_1, \event_2, \trace, c, D) $, then
 $z_1^{r_1}, \cdots, z_n^{r_n} \in \lvar_{{c}}$ with $n \geq 0$ such that   
$\flowsto(x^i,  z_1^{r_1}, c) 
\land \cdots \land \flowsto(z_n^{r_n}, y^j, c)$
%
\[
  \begin{array}{l}
		\forall D \in \dbdom , c \in \cdom, \trace \in \mathcal{T} \st \forall \event_1, \event_2 \in \eventset \st
    \event_1, \event_2 \in \eventset^{\asn} \land 
		 \exists \trace' \in \mathcal{T} \st \trace = [\event_1] \tracecat \trace' \tracecat [\event_2]
		\implies
		\eventdep(\event_1, \event_2, \trace, c, D) 
		\\ \quad 
		\implies 
    \exists n \in \mathbb{N}, z_1^{r_1}, \cdots, z_n^{r_n} \in \lvar_{{c}} \st n \geq 0 \land
		\flowsto(\pi_1(\event_1)^{\pi_2(\event_1)},  z_1^{r_1}, c) 
    \land \cdots \land \flowsto(z_n^{r_n}, \pi_1(\event_2)^{\pi_2(\event_2)}, c) 
	\end{array}
\]
\end{thm}
Proof Summary:
I. Vacuously True cases, where trace doesn't satisfy the hypothesis 
\\
II. Base case where $\trace = [\event_1;\event_2]$
\\
III. inductive case where $\trace = [\event_1, \cdots, \event_2]$.
\\
1. Existence of a middle event:
\\
Proved by showing a contradiction, with detail in Lemma~\ref{lem:depevents_exist}.
%
\\
2. The middle event with a sub-trace implies a "sub flowsto-chain", informally:
%
\\
(1). obtaining the existence of $\event_z \in \eventset^{\asn} $ with dependency on $\event_x$, and a "direct flowsto" from $\event_z$ to $\event_y$
by Lemma~\ref{lem:depevents_exist}.
 \\
(2). from the dependency of the $\event_z$ with $\event_x$ on the subtrace,
 obtaining a "sub flowsto-chain" by induction  hypothesis;
 \\
(3). composing the "sub flowsto-chain" from (2) with the  "direct flowsto" from (1), and getting the conclusion of
 the complete "flowsto chain".
%
\begin{proof}
  Taking arbitrary $D \in \dbdom , c \in \cdom,$ by induction on the trace $\trace$ we have the following cases:
  \begin{case}($\trace = {[]}$)
    \\
    Since for all $\event_1, \event_2 \in \eventset^{\asn}$,
     $\not\exists \trace' \in \mathcal{T}$,satisfies $
    {[]}  = [\event_1] \tracecat \trace' \tracecat [\event_2]$, the theorem is vacuously true.
    \end{case}
    %
    \begin{case}($\event \in \eventset, \trace = [\event]$)
    \\
    Since for all $\event_1, \event_2 \in \eventset^{\asn}$,
     $\not\exists \trace' \in \mathcal{T}$,satisfies $
    {[]} = [\event_1] \tracecat \trace' \tracecat [\event_2]$, the theorem is vacuously true.
    \end{case}
    %
    \begin{case}
      \label{case:soundness_basecase}
      ($\event_1', \event_2' \in \eventset $, $\trace = [\event_1'; \event_2']$)
      \\
      To show:
      % \wq{$\forall l \in \mathcal{A}(\event_1, \event_2, \trace, c, D)$ below?}
      %\jl{yes, there is a typo}
      \[
      \begin{array}{l}
        \forall \event_1, \event_2 \in \eventset^{\asn} \st
        \exists \trace' \in \mathcal{T} \st [\event_1'; \event_2'] = [\event_1] \tracecat \trace' \tracecat [\event_2]
        \\ \qquad 
            \implies    
        % \forall  z^i, y^j \in \lvar_c, l_h, l_t \st 
          \eventdep(\event_1, \event_2, [\event_1; \event_2], c, D)
         \implies \flowsto(\pi_1(\event_1)^{\pi_2(\event_1)}, \pi_1(\event_2)^{\pi_2(\event_2)}, c)
      \end{array}
      \]
      %
      Taking arbitrary $ \event_1, \event_2 \in \eventset^{\asn}$, by law of excluded middle, there are 2 cases:
      \\
      $\event_1 = \event_1' \land  \event_2 = \event_2'$
      \\
      $\neg(\event_1 = \event_1' \land  \event_2 = \event_2')$
      \\
      In case of $\neg(\event_1 = \event_1' \land  \event_2 = \event_2')$, since 
      $\not\exists \trace' \in \mathcal{T}$,satisfies $
      [\event_1'; \event_2'] = [\event_1] \tracecat \trace' \tracecat [\event_2]$, 
      the theorem is vacuously true.
      \\
      %
      In case of $\event_1 = \event_1' \land  \event_2 = \event_2'$,
      let $\trace' = []$, we know $\exists \trace' \in \mathcal{T}$ satisfying 
      $[\event_1; \event_2] = [\event_1] \tracecat \trace' \tracecat [\event_2]$.
      \\
      % By Inversion Lemma~\ref{lem:inv_alg2}, we have either one of the two following cases:
      % \begin{enumerate}
      %   \item $\mathcal{A}(\event_1, \event_2, [\event_1; \event_2], c, D) = 
      %   \left\{[\pi_1(\event_1)^{\pi_2(\event_1)}, \pi_1(\event_2)^{\pi_2(\event_2)}] \right \}$ 
      %   and $\eventdep(\event_1, \event_2, \cdot  \event_1 \cdot \event_2, c, D)$.
      %   \item  $\mathcal{A}(\event_1, \event_2, [\event_1; \event_2], c, D) = \{\}$ 
      %   and $\neg \eventdep(\event_1, \event_2, \cdot  \event_1 \cdot \event_2, c, D)$;
      % \end{enumerate}
      % %
      % In case of $\mathcal{A}(\event_1, \event_2, [\event_1; \event_2], c, D) = \{\}$,
      % since $\not\exists  z^i, y^j \in \lvar_c, l_h, l_t \st l_h ++ [z^i, y^j] ++ l_t \in \{\}$, the theorem is vacuously true.
      % %
      % \\
      % Then in the case 1., 
      Then it is sufficient to show: 
      % \wq{Because $l \in A \implies DEP$ }
      % \jl{yes}
      \[
        \eventdep(\event_1, \event_2, [\event_1; \event_2], c, D) 
        \implies \flowsto(\pi_1(\event_1)^{\pi_2(\event_1)}, \pi_1(\event_2)^{\pi_2(\event_2)}, c)
        % \land \eventdep(\event_1, \event_2, \cdot  \event_1 \cdot \event_2, c, D)
      \]
      %
     By Lemma~\ref{lem:flowsto_soundness_emptytrace}, we have this case proved.
      %
      \end{case}
      %
        %
        \begin{case}
        ($\event_1', \event_2' \in \eventset$, $\trace_{ih} \in \mathcal{T}, \trace = [\event_1'] \tracecat \trace_{ih} \tracecat [\event_2'] \land \trace_{ih} \neq {[]}$)
        \\
        It is sufficient to show:
        \[    \begin{array}{l}
         \forall \event_1, \event_2 \in \eventset \st
          \event_1, \event_2 \in \eventset^{\asn} \land 
           \exists \trace' \in \mathcal{T} \st \trace = [\event_1] \tracecat \trace' \tracecat [\event_2]
          \implies
          \eventdep(\event_1, \event_2, [\event_1'] \tracecat \trace_{ih} \tracecat [\event_2'], c, D) 
          \\ \quad 
          \implies 
          \exists n \in \mathbb{N}, z_1^{r_1}, \cdots, z_n^{r_n} \in \lvar_{{c}} \st n \geq 0 \land
          \flowsto(\pi_1(\event_1)^{\pi_2(\event_1)},  z_1^{r_1}, c) 
          \land \cdots \land \flowsto(z_n^{r_n}, \pi_1(\event_2)^{\pi_2(\event_2)}, c) 
        \end{array}
        \]
        %
        with the induction hypothesis:
        %
        \[
          \begin{array}{l}
            \forall \event_{ih1}, \event_{ih2} \in \trace \st \event_{ih1}, \event_{ih2} \in \eventset^{\asn} 
            \land
             \exists \trace' \in \mathcal{T} \st 
             \trace[\event_{ih1}:\event_{ih2}] = [\event_{ih1}] \tracecat \trace' \tracecat [\event_{ih2}]
            \implies
            \eventdep(\event_{ih1}, \event_{ih2}, \trace[\event_{ih1}:\event_{ih2}], c, D) 
            \\ \quad 
            \implies 
            \exists n \in \mathbb{N}, z_1^{r_1}, \cdots, z_n^{r_n} \in \lvar_{{c}} \st n \geq 0 \land
            \flowsto(\pi_1(\event_{ih1})^{\pi_2(\event_{ih1})},  z_1^{r_1}, c) 
            \land \cdots \land \flowsto(z_n^{r_n}, \pi_1(\event_{ih2})^{\pi_2(\event_{ih2})}, c) 
          \end{array}
        \]
        %
        %
        Taking arbitrary $ \event_1, \event_2 \in \eventset^{\asn}$, by law of excluded middle, there are 2 cases:
        \\
        $\event_1 = \event_1' \land  \event_2 = \event_2'$
        \\
        $\neg(\event_1 = \event_1' \land  \event_2 = \event_2')$
        \\
        In case of $\neg(\event_1 = \event_1' \land  \event_2 = \event_2')$, since 
        $\not\exists \trace' \in \mathcal{T}$,satisfies $
        [\event_1'] \tracecat \trace_{ih} \tracecat [\event_2']  = [\event_1] \tracecat \trace' \tracecat [\event_2]$, 
        the theorem is vacuously true.
        \\
        %
        In case of $\event_1 = \event_1' \land  \event_2 = \event_2'$,
        let $\trace' = \trace_{ih}$, we know $\exists \trace' \in \mathcal{T}$ satisfying 
        $[\event_1'] \tracecat \trace_{ih} \tracecat [\event_2'] = [\event_1] \tracecat \trace' \tracecat [\event_2]$.
        \\
        To show:
        \[
          \begin{array}{l}
            \eventdep(\event_1, \event_2, [\event_1] \tracecat \trace_{ih} \tracecat [\event_2], c, D) 
          \\ \quad 
          \implies 
          \exists n \in \mathbb{N}, z_1^{r_1}, \cdots, z_n^{r_n} \in \lvar_{{c}} \st n \geq 0 \land
          \flowsto(\pi_1(\event_1)^{\pi_2(\event_1)},  z_1^{r_1}, c) 
          \land \cdots \land \flowsto(z_n^{r_n}, \pi_1(\event_2)^{\pi_2(\event_2)}, c) 
        \end{array}
        \]
        %
        By Lemma~\ref{lem:depevents_exist}, we know:
        \[
          \begin{array}{l}
            \flowsto(\pi_1(\event_1)^{\pi_2(\event_1)}, \pi_1(\event_2)^{\pi_2(\event_2)}, c) 
        \\ \qquad \quad \lor
        \exists \event \in \trace_{ih} \st 
        % \left( 		
          \eventdep(\event_1, \event, \trace[\event_1:\event], c, D)
        \land 
        \flowsto(\pi_1(\event)^{\pi_2(\event)}, \pi_1(\event_2)^{\pi_2(\event_2)}, c) 
      \end{array}
      \]
        \\
        In first case, we have $\flowsto(\pi_1(\event_1)^{\pi_2(\event_1)}, \pi_1(\event_2)^{\pi_2(\event_2)}, c) $ proved directly.
        \\
        In the second case, let $\event_{ih}$ be this event, from the induction hypothesis, we know:
        \[
          \exists n \in \mathbb{N}, z_1^{r_1}, \cdots, z_n^{r_n} \in \lvar_{{c}} \st n \geq 0 \land
            \flowsto(\pi_1(\event_1)^{\pi_2(\event_1)},  z_1^{r_1}, c) 
            \land \cdots \land \flowsto(z_n^{r_n}, \pi_1(\event_{ih})^{\pi_2(\event_{ih})}, c) 
          \]
          % \\
          Then we know:
          \[
            \begin{array}{l}
              \exists n \in \mathbb{N}, z_1^{r_1}, \cdots, z_n^{r_n} \in \lvar_{{c}} \st n \geq 0 \land
            \flowsto(\pi_1(\event_1)^{\pi_2(\event_1)},  z_1^{r_1}, c) 
            \land \cdots \land \flowsto(z_n^{r_n}, \pi_1(\event_{ih})^{\pi_2(\event_{ih})}, c) )
             \\ \quad  
             \land  \flowsto(\pi_1(\event)^{\pi_2(\event)}, \pi_1(\event_2)^{\pi_2(\event_2)}, c) 
            \end{array}
            \]
            This case is proved.
      \end{case}
      %
  % \[
  %   \begin{array}{l}
  %     \forall D \in \dbdom , c \in \cdom, \trace \in \mathcal{T} \st \forall \event_1, \event_2 \in \eventset \st
  %     \event_1, \event_2 \in \eventset^{\asn} \land 
  %      \exists \trace' \in \mathcal{T} \st \trace = [\event_1] \tracecat \trace' \tracecat [\event_2]
  %     \implies
  %     \eventdep(\event_1, \event_2, \trace, c, D) 
  %     \\ \quad 
  %     \implies 
  %     \exists n \in \mathbb{N}, z_1^{r_1}, \cdots, z_n^{r_n} \in \lvar_{{c}} \st n \geq 0 \land
  %     \flowsto(\pi_1(\event_1)^{\pi_2(\event_1)},  z_1^{r_1}, c) 
  %     \land \cdots \land \flowsto(z_n^{r_n}, \pi_1(\event_2)^{\pi_2(\event_2)}, c) 
  %   \end{array}
  % \]

%
\end{proof}

\subsection{Inversion Lemmas and Helper Lemmas}
The following are the inversion lemmas and helper lemmas used in the proof of Theorem~\ref{thm:flowsto_event_soundness} above,
showing the correspondence properties between the trace based semantics and the program analysis results.
\input{lem_depinversion}