\[
\begin{array}{ll}
 F(\expr, \phi ) & where \eapp ~~ \phi(x_i) = (\idx_i, \adapt_i, \nnatA_i ) \\
   F(x,\phi) & = \sum_{x_i \in \fv{x}  } \idx_i \times (\adapt_i+ \nnatA_i)  \\
F(\lambda x. \expr ,  \phi  ) & =  \sum_{x_i \in \fv{\lambda x.\expr}  } \idx_i \times (\adapt_i+ \nnatA_i)   \\  %\sum_{x_i \in \fv{\lambda x.\expr} } k_i \times R_i  \\
F(\delta(\expr) , \phi ) & = \sum_{x_i \in \fv{\delta(\expr)} } \idx_i \times (\adapt_i+ \nnatA_i)  \\
F(c, \phi ) & = 0  \\
F(\expr_1 \eapp \expr_2, \phi ) & = F(\expr_1, \phi ) +
                                  F(\expr_2,\phi ) \\
F(\eif \expr \ethen \expr_1 \eelse \expr_2, \phi ) & = F(\expr, \phi) + \max(F(\expr_1, \phi),  F(\expr_2, \phi)   )  
\end{array} 
\]

\begin{defn}[Typable]
  \label{typable}
  A closure $( \expr, [ x_1 \to (\valr_1 ,  \env_1 , \adapt_1 ) , \ldots, x_i \to (\valr_i, \env_i, \adapt_i )] )$ is typable with type $\type$ and adaptivity $J$ if exists $k_i$\\
  \[
     x_1 : \bang{\idx_1} \type_1, \ldots, \bang{\idx_i} \type_i 
     \tvdash{\nnatA}  \expr : \type  \]
   and each closure $(\valr_i, \env_i)$  is also typable with type $\bang{\idx_i} \type_i$ and adaptivity $\nnatA_i$, $ \phi = [x_1
     \to (\idx_1, \adapt_1, \nnatA_1), \ldots,  x_i \to (\idx_i, \adapt_i,
     \nnatA_i)  ] $,  $J = \nnatA + F( \expr, \phi ) $.
 \end{defn}

 \begin{defn}[ClosedClosure]
  \label{closure}
   A closure $(\expr, \env)$ is closed if $\fv{\expr} \subseteq \dom(\env)$. 
 \end{defn}

% \begin{lem}[ClosureTypable ]
%   \label{ct}
%    If a closure $(\expr, \env)$ is closed, then there exists $\type$ and $J$ so that $(\expr, \env)$ is typable with $\type$ and $J$.
%    \end{lem}
 

\begin{lem}[programTypable]
  \label{proglemma}
   If $ \tvdash{\nnatA}   \expr : \type $, then $(
     \expr, \emptyset ) $ is typable with $\type$ and adaptivity $\nnatA$. 
   \end{lem}

   \begin{lem}[TypableMono]
     \label{tmono}
     If a closure is $D$ is typable with $\type$ and $\nnatA$, and $\nnatA \leq \nnatA'$, then
     D is typable with $\type$ and $\nnatA'$.
    \end{lem} 

   
\begin{lem}[TypableSoundness]
  \label{tsound}
  If a closure $D$ is typable with $\type$ and $J$, and $D \bigstep{\adapt} E$, then
    closure $E$ is typable with $\type$ and adaptivity $J - \adapt$. 
   \end{lem}

   \begin{proof}
     By induction on the evaluation semantics.\\

     \caseL{Case
       \[
         \inferrule{  \env(x)  =  (\valr, \env',  \adapt)  }
         {x,\env  \bigstep{\adapt} \valr, \env' }~\textsf{var2}
       \]
     }

     Suppose $(x,\env)$ is typable with $\type$ and $J$ and $\env = [x \to (\valr, \env', \adapt), x_1 \to (\valr_1, \env_1, \adapt_1) , \ldots ,  x_i \to (\valr_i, \env_i, \adapt_i) ]  $\\
     
     We know that: exists $k_i$ so that $ x_1 : \bang{\idx_1} \type_1, \ldots, \bang{\idx_i} \type_i,  x: \bang{1} \type \tvdash{0} x : \type $,  and the each closure $ (\valr_i, \env_i) $ is typable with $\type_i$ and $\nnatA_i$ as well as $(\valr, \env')$ is typable with $\type$ and $\nnatA$.  and $J = 0 + (\adapt + \nnatA) $.\\

     TS: $(\valr, \env') $ is typable with $\type$ and $J - \adapt$,  it is proved by Lemma~\ref{tmono} on the assumption.\\

     \caseL{Case
       \[
         \inferrule{
    \expr_1, \env_1 \bigstep{\adapt_1} \lambda x.\expr , \env_1' \\
    %\forall x_i \in \dom(\env_1 \cap \env_2).  \fresh \eapp x_i' \\
     \expr_2, \env_2 \bigstep{\adapt_2} \valr_2 , \env_2' \\
    \fresh \eapp x' \\
    \expr[x'/x], \env_1'[ x'  \to (\valr_2, \env_2', \adapt_2  ) ] 
    \bigstep{\adapt_3} \valr, \env_3 ~(\clubsuit)
  }{
     \expr_1 \eapp \expr_2 , (\env_1 \uplus \env_2)\bigstep{\adapt_1+\adapt_3} \valr, \env_3
  }~\textsf{app}
     \]
   }
   
   Suppose for each variable $x_i \in \dom(\env_1)$, $(\valr_i, \env_i)$ is tyable with type $\type_i$ and $I_i$. For each variable $x_j \in \dom(\env_2)$, $(\valr_j, \env_j)$ is tyable with type $\type_j$ and $I_j$.
   
   We assume exists $\idx_i$ and $\Gamma_1 = x_1 : \bang{\idx_1} \type_1 , \ldots, x_i : \bang{\idx_i} \type_i$ for $x_i \in \dom(\env_1)$, so that $  \Gamma_1  \tvdash{\nnatA_1} \expr_1:  \bang{\idx} \type_1 \lto{\nnatA} \type_2 $.

   Similarly, we assume exists $\idx_j$ and $\Gamma_2 = x_1 : \bang{\idx_1} \type_1 , \ldots, x_j : \bang{\idx_j} \type_j$ for $x_j \in \dom(\env_j)$, so that $\Gamma_2 \tvdash{\nnatA_2} \expr_2: \type_1$.
  
   By the typing rule app, we have:  
   \[
     \inferrule{
      \ictx \Gamma_1  \tvdash{\nnatA_1} \expr_1:  \bang{\idx} \type_1
      \lto{\nnatA} \type_2      \\
      \ictx \Gamma_2 \tvdash{\nnatA_2} \expr_2: \type_1 
    }{
      \ictx   \Gamma_1 + \idx \times \Gamma_2  \tvdash{    \nnatA_1 +
        \idx \times \nnatA_2 + \nnatA    } \expr_1 \eapp \expr_2 : \type_2
    }~\textbf{app}
  \]

  We know that $\dom(\Gamma_1 + \idx \times \Gamma_2) = \dom(\Gamma_1) \cup \dom(\Gamma_2) = \dom( \env_1 \uplus \env_2 )$. So forall all the closure $(\valr_i, \env_i)$ assigned by variable $x_i \in \dom(\Gamma_1 + \idx \times \Gamma_2)$,  $(\valr_i, \env_i)$ is typable with $\type_i$ and $I_i$ from our assumption.

  $\phi = [x_1 \to (\idx_1, \adapt_1, I_1) , \ldots, x_i \to (\idx_i, \adapt_i, I_i)]$ where $x_i \in \dom(\env_1 \uplus \env_2)$.

  So, we know that : $( \expr_1 \eapp \expr_2,  \env_1 \uplus \env_2 )$ is typable with $\type_2$ and $J= \nnatA_1 +\idx \times \nnatA_2 + \nnatA   +F(\expr_1 \eapp \expr_2, \phi) $. \\
   
   TS: $(\valr, \env_3) $ is typable with  $\type_2$ and $J- (\adapt_1+\adapt_3)$.

   Set $\phi_1 =[x_1 \to (\idx_1, \adapt_1, I_1) , \ldots, x_i \to (\idx_i, \adapt_i, I_i)]$ where $x_i \in \dom(\env_1)$.

    Set $\phi_2 =[x_1 \to (\idx_1, \adapt_1, I_1) , \ldots, x_i \to (\idx_i, \adapt_i, I_i)]$ where $x_i \in \dom(\env_2)$.
   
   From our assumption, we also know that $(\expr_1, \env_1)$ is typable with $\bang{\idx} \type_1 \lto{\nnatA} \type_2$ and $J_1 = \nnatA_1 +   F(\expr_1, \phi_1) $.

   Similarly, we have: $(\expr_2, \env_2)$ is  typable with $\type_1$ and $J_2 = \nnatA_2 + F(\expr_2, \phi_2)$ for $x_j \in \dom(\env_2)~(2)$ .

   By induction hypothesis on $(1)$, $(2)$ respectively, we know that:
   
   $ ( \lambda x.\expr , \env_1') $ is typable with $\bang{\idx} \type_1 \lto{\nnatA} \type_2$ and $J_1 - \adapt_1$ ~(3). 
   
   $(\valr_2 , \env_2')  $ typable with $ \type_1 $ and $J_2 -\adapt_2$ (4). 

   From (3), we know the following if we assume exists $\idx_i''$ and $\Gamma_1'' = x_1'' : \bang{\idx_1''} \type_1'', \ldots, x_i'' : \bang{\idx_i''} \type_i'' $, and $\env_1'(x_i'') = (\valr_i'', \env_i'', \adapt_i'')$ and each closure $(\valr_i'', \env_i'' )  $ is typable with $\type_i''$ and $I_i''$.

 Set $\phi_1'' =[x_1'' \to (\idx_1'', \adapt_1'', I_1'') , \ldots, x_i'' \to (\idx_i'', \adapt_i'', I_i'')]$ where $x_i'' \in \dom(\env_1')$.

   
   $$ \inferrule{
      \ictx \Gamma_1'', x: \bang{\idx} \type_1
      \tvdash{\nnatA }
      \expr: \type_2 ~(\star)
    }{
      \ictx \Gamma_1'' \tvdash{0} \lambda x. \expr : \bang{\idx} \type_1
      \lto{\nnatA} \type_2
    }~\textbf{lambda} $$
    and we know $J_1 - \adapt_1 = 0 + F(  \lambda x. \expr , \phi_1'' )$.

    Take a fresh variable $x'$, from $(\star)$, we know: $\ictx \Gamma_1, x': \bang{\idx} \type_1 \tvdash{\nnatA }  \expr[x/x']: \type_2 ~(\star\star) $.
    
   Set $\phi_1''' = \phi_1''[x' \to (\idx, \adapt_2,  J_2-\adapt_2 )]$.
    
   From $(\star\star)$ and $(4)$, we conclude that $( \expr[x'/x], \env_1'[ x'  \to (\valr_2, \env_2', \adapt_2  ) ] )$ is typable with $\type_2$ and $ \nnatA+ F( \expr[x'/x], \phi_1''' )$.

Because  $ F( \expr[x'/x], \phi_1''' ) =   F(\lambda x.\expr, \phi_1'') +\idx \times (\adapt_2 + J_2 -\adapt_2 ) = J_1 - \adapt_1 + \idx \times  J_2$.

    By induction hypothesis using $(\clubsuit)$ and the above statement, we know:
    $\valr, \env_3$ is typable with $\type_2$ and $\nnatA + J_1 - \adapt_1 +\idx \times  J_2 - \adapt_3$.

    Unfold $J_1, J_2$, we know 
    $ \nnatA + J_1 - \adapt_1 +\idx \times  J_2 - \adapt_3  = \nnatA + \nnatA_1 + F(\expr_1, \phi_1)  + \idx \times \nnatA_2 + \idx \times F(\expr_2, \phi_2)  - (\adapt_1 + \adapt_3) \leq  J- (\adapt_1+\adapt_3) $.

    The TS is proved by lemma~\ref{tmono} on the above statement.

    \caseL{Case
      \[
         \inferrule{
  \expr , \env \bigstep{\adapt} \efalse, \env'
   \\
    \expr_2 , \env \bigstep{\adapt_2} \valr_2, \env_2
  }{
    \eif \expr \ethen \expr_1 \eelse \expr_2 , \env \bigstep{\adapt +
      \adapt_2 } \valr_2, \env_2
  }~\textsf{if-f}
      \]
    }

    Assume for all the variables $x_i \in \dom(\env)$, $ \env(x_i) = (\valr_i, \env_i, \adapt_i)$ and $(\valr_i, \env_i)$ is typable with $\type_i$ and $I_i$.
    
    We assume exists $\Gamma' = x_1 : \bang{\idx_1} \type_1 , \ldots, x_i: \bang{\idx_i} \type_i$ and $\dom(\Gamma') = \dom(\env)$, and assume the follwoing using the typing rule if.

    \[
      \inferrule{
      \ictx \Gamma \tvdash{\nnatA} \expr: \tbool ~(\star)
      \\
      \ictx \Gamma_1 \tvdash{\nnatA_1} \expr_1: \type
      \\
       \ictx \Gamma_2 \tvdash{\nnatA_2} \expr_2: \type ~(\diamond)
      \\
      \Gamma' = \Gamma + \Gamma_1 + \Gamma_2
      \\
      \nnatA' = \nnatA + \max(\nnatA_1, \nnatA_2)
    }{
      \ictx \Gamma' \tvdash{\nnatA'}  \eif \expr  \ethen \expr_1 \eelse \expr_2 : \type 
    }~\textbf{if}
  \]
  
Set $\phi = [x_1 \to (\idx_1, \adapt_1, I_1) , \ldots, x_i \to (\idx_i, \adapt_i, I_i)]$ where $x_i \in \dom(\env)$.

  We have :  $(\eif \expr \ethen \expr_1 \eelse \expr_2 , \env )$ is typable with $\type$ and $J$, where $J = \nnatA' + F(\eif \expr \ethen \expr_1 \eelse \expr_2, \phi )$

  TS: $(\valr_2, \env_2 )$ is typable with $\type$ and $J-(\adapt + \adapt_2)$.
  
  From $(\star)$, we know from weaking rule that $\Gamma, x_j: \bang{0} \type_j \tvdash{\nnatA} \expr: \tbool ~(1) $ where $x_j \in \dom(\env) \setminus \dom(\Gamma) $.

  Set $\phi_1 = [x_1 \to (\idx_1, \adapt_1, I_1) , \ldots, x_i \to (\idx_i, \adapt_i, I_i)]$ where $\idx_j = 0 $ for $x_j \in \dom(\env) \setminus \dom(\Gamma) $.

  Similaly, from $(\diamond)$, we have  $ \Gamma_2, x_j: \bang{0} \type_j \tvdash{\nnatA_2} \expr_2: \type ~(2)$  where $x_j \in \dom(\env) \setminus \dom(\Gamma_2) $.

   Set $\phi_2 = [x_1 \to (\idx_1, \adapt_1, I_1) , \ldots, x_i \to (\idx_i, \adapt_i, I_i)]$ where $\idx_j = 0 $ for $x_j \in \dom(\env) \setminus \dom(\Gamma_2) $.
  
   From $(1)$, we know that $(\expr, \env )$ is typable with $\tbool$ and $J_1$, where $J_1 = \nnatA + F(\expr, \phi_1 )~(3)$.

    From $(2)$, we know that $(\expr_2, \env )$ is typable with $\type$ and $J_2$, where $J_2 = \nnatA_2 + F(\expr_2, \phi_2 )~(4)$.

    By IH on $(3)$, $(4)$, we have $(\efalse, \env_1')$ is typable with $\tbool$ and $J_1 - \adapt~(5)$ and $(\valr_2, \env_2)$ is typable with $\type$ and $J_2 - \adapt_2(6)$.

    we know that $ J = \nnatA' +  F(\eif \expr \ethen \expr_1 \eelse \expr_2, \phi )  = \nnatA + F(\expr, \phi) + \max(\nnatA_1, \nnatA_1) + \max(F(\expr_1, \phi) , F(\expr_2, \phi) )  \geq (J_1 + J_2) $.

     We also know $J_1 -\adapt \geq 0$ from $(5)$, 

    So we know $ J - (\adapt + \adapt_2) \geq (J_1 + J_2) - (\adapt+\adapt_2) \geq J_2 - \adapt_2 $.  Our TS can be proved using Lemma~\ref{tmono} on $(6)$.
  
    
   \end{proof}  