\begin{defn}[Typable Closures]
  \label{def:typable}
Let $\env=[ x_1 \to (\valr_1 ,  \env_1 , R_1 ) ,
  \ldots, x_n \to (\valr_n, \env_n, R_n )]$. 
  The closure $( \expr, \env)$ is typable with
  type $\type$ and adaptivity $J$ if:
\begin{enumerate}\item  
     $x_1 : \bang{k_1} \type_1, \ldots, \bang{k_i} \type_i 
     \tvdash{Z}  \expr : \type$, for some types $\bang{k_i}
   \type_i$ for $(1\leq i\leq n)$, 
\item each closure $(\valr_i, \env_i)$ for $(1\leq i\leq n)$ is typable with type
  $\bang{k_i} \type_i$ and adaptivity $Z_i$,
\item $J = Z + \sum_{(v_i,\theta_i,S_i)\in\theta} k_i \times (R_i
  +Z_i)$.
\end{enumerate}
 \end{defn}
To justify why we chose $\sum$ in the third clause above it is worth
to consider the following configuration:
$$
[x\mapsto (\lambda u.\lambda w.\delta(u)+\delta(w),[\,],0)
,y:\mapsto (v,[\,],2) ], x\, y\, y
$$
\mg{To elaborate the example above}
   
\begin{lem}[Soundness]
  \label{tsound}
  If a closure $D$ is typable with type $\type$ and adaptivity $J$, and $D \bigstep{R} E$, then
    the closure $E$ is typable with type $\type$ and adaptivity $I$,
    where $I+R\leq J$. 
   \end{lem}

   \begin{proof}
     By induction on the derivation showing $D \bigstep{R} E$. The
     rules \textsf{lambda},\textsf{val}, and \textsf{const} dollow
     from the hypothesis. We will discuss the other cases. \\

     \caseL{Case
       \[
         \inferrule{  \env(x)  =  (\valr, \env',  R)  }
         {x,\env  \bigstep{R} \valr, \env' }~\textsf{var}
       \]
     }

     By assumption, the closure $(x,\env)$ is typable with type
     $\type$ and adaptivity $J$. Let us assume without loss of
     generality that
     $\env=[x\to (\valr , \env' , R ), x_1 \to (\valr_1 , \env_1 , R_1 ) , \ldots, x_n \to
     (\valr_n, \env_n, R_n )]$.  By Definition~\ref{def:typable} we have that
     there exist $k$ and $\bang{k_i} \type_i$ for $(1\leq i\leq n)$ such
     that:
     \[ x: \bang{k}\type, x_1 : \bang{k_1} \type_1, \ldots, x_n:\bang{k_n} \type_n \tvdash{Z} x : \type \]
    Moreover, we have that the closure $(\valr,\env')$ is typable with
    type $\type$ and adaptivity $I$, and that each closure $ (\valr_i, \env_i) $ is
    typable with type $\type_i$ and adaptivity $Z_i$, and that 
$$J = Z + k\times (R+I)+ \sum_{1\leq
  i\leq n, i\neq j} k_i \times (R_i
  +Z_i).$$
By inversion on the typing rules, we have that $k= 1$, hence
we can rewrite $J$ as 
$$J = Z + R+I+ \sum_{1\leq
  i\leq n, i\neq j} k_i \times (R_i
  +Z_i)).$$
Hence, it is easy to see that $ I+R\leq J$ which is
what we need to show.\\


     \caseL{Case
       \[
         \inferrule{
    \expr_1, \env \bigstep{R_1} \lambda x.\expr , \env^1 \\
    %\forall x_i \in \dom(\env_1 \cap \env_2).  \fresh \eapp x_i' \\
     \expr_2, \env \bigstep{R_2} \valr_2 , \env^2 \\
    \fresh \eapp x' \\
    \expr[x'/x], \env^1[ x'  \to (\valr_2, \env^2, R_2  ) ] 
    \bigstep{R_3} \valr, \env^3 ~(\clubsuit)
  }{
     \expr_1 \eapp \expr_2 , \env\bigstep{R_1+R_3} \valr, \env^3
  }~\textsf{app}
     \]
   }
   By assumption, the closure $(\expr_1 \eapp \expr_2 , \env)$ is
   typable with type $\tau$ and adaptivity $J$.  Let us assume without
   loss of generality that
   $\env=[x_1 \to (\valr_1 , \env_1 ,
   S_1 ) , \ldots, x_n \to (\valr_n, \env_n, S_n )]$.  By
   Definition~\ref{def:typable} we have that there exist 
   $\bang{k_i} \type_i$ for $(1\leq i\leq n)$ such that:
     \begin{equation}
\label{fact:app}
       x_1 : \bang{k_1} \type_1, \ldots, x_n:\bang{k_n} \type_n
       \tvdash{Z} \expr_1\expr_2 : \type 
\end{equation}
    Moreover, we have that each closure $ (\valr_i, \env_i)\in\theta $ is
    typable with type $\type_i$ and adaptivity $Z_i$, and that 
$$J = Z + \sum_{(v_i,\theta_i,S_i)\in\theta} k_i \times (S_i
  +Z_i).$$
By inversion on Fact~\ref{fact:app} we have that there exist
$\sigma,Z',Z^1, k$ and $k_i^1$ for $(1\leq i\leq n)$ such that:
\begin{equation}
\label{fact:head}
 x_1 : \bang{k_1^1} \type_1, \ldots, x_n:\bang{k_n^1} \type_n
       \tvdash{Z^1} \expr_1 : \bang{k} \sigma
      \lto{Z'} \type
\end{equation}
Similarly, 
we have that there exist
$Z^2$ and $k_i^2$ for $(1\leq i\leq n)$ such that:
\begin{equation}
\label{fact:arg}
 x_1 : \bang{k_1^2} \type_1, \ldots, x_n:\bang{k_n^2} \type_n
       \tvdash{Z^2} \expr_2 : \sigma
\end{equation}
Moreover, we have that $Z=Z^1+k\times Z^2+Z'$, and that
$k_i=k_i^1+k\times k_i^2$.  

Using  Fact~\ref{fact:head} and the assumption
that each closure $ (\valr_i, \env_i) $ in $\theta$ is typable with
type $\type_i$ and adaptivity $Z_i$ we have that the closure
$(e_1,\theta)$ is typable with type $\bang{k} \sigma
      \lto{Z'} \type$ and adaptivity:
$$
Z^1+\sum_{(v_i,\theta_i,S_i)\in\theta}k_i^1\times(S_i+Z_i)
$$
By induction hypothesis we then have that the closure 
$(\lambda x. e,\theta^1)$ is typable with type $\bang{k} \sigma
      \lto{Z'} \type$ and adaptivity $I_1$ where 
$$I_1+R_1\leq Z^1+\sum_{(v_i,\theta_i,S_i)\in\theta }k_i^1\times(S_i+Z_i)$$
It is worth to stress here that by definition, using the fact that 
$$
 x_1 : \bang{k_1^1} \type_1, \ldots, x_n:\bang{k_n^1} \type_n
       \tvdash{0} \lambda x. \expr : \bang{k} \sigma
      \lto{Z'} \type
$$
which follows from Fact~\ref{fact:head} and inversion on the rule {\bf
  lambda} \mg{here we actually want a lemma that says that values are typable
  with $\vdash_0$, and that takes care of the free variables that we may
  have added} we have:
$$
I_1=\sum_{(v_i,\theta_i,S_i)\in\theta^1}k_i^1\times(S_i+Z_i)
$$
%
Using  Fact~\ref{fact:arg} and again the assumption
that each closure $ (\valr_i, \env_i) $ in $\theta$ is typable with
type $\type_i$ and adaptivity $Z_i$ we have that the closure
$(e_2,\theta)$ is typable with type $\type$ and adaptivity:
$$
Z^2+\sum_{(v_i,\theta_i,S_i)\in\theta}k_i^2\times(S_i+Z_i)
$$

By induction hypothesis we than have that the closure 
$(v_2,\theta_2)$ is typable with type $\type$ and adaptivity $I_2$ where 
$$I_2+R_2\leq Z^2+\sum_{(v_i,\theta_i,S_i)\in\theta}k_i^2\times(S_i+Z_i)$$
%
It is again worth to stress here that by definition, using the fact
that $v_2$ is a value we have:
$$
I_2=\sum_{(v_i,\theta_i,S_i)\in\theta^2}k_i^2\times(S_i+Z_i)
$$
By Fact~\ref{fact:head}, and type preservation and some other Lemma
\mg{TODO: we need to be more clear and handle the fact that the adaptivity can be 0 in the
lambda rule} we have 
\begin{equation}
\label{fact:reduct}
 x_1 : \bang{k_1^1} \type_1, \ldots, x_n:\bang{k_n^1} \type_n,
       x: \bang{k} \sigma\tvdash{{Z'}} \expr : 
       \type
\end{equation}
By composing this with the previous assumptions, we have that the closure 
$(e[x'/x],\theta^1[x'\mapsto (v_2,\theta_2,R_2)])$ is typable with
type $\type$ and adaptivity $I_3$ where 
$$I_3=Z'+k\times(R_2+I_2)+\sum_{(v_i,\theta_i,S_i)\in\theta^1}k_i^1\times(S_i+Z_i)$$
By induction hypothesis we then get that the closure $(v,\theta^3)$ is
typable with type $\type$ and adaptivity $I$ where $I+R_3\leq
I_3$. Notice also that we have a $\theta^4$ such that
$\theta^3=\theta^4[x' \mapsto (v_2,\theta_2,R_2) ]$.
Moreover, once again, note that by Lemma~\mg{Lemma showing that we can
  type values with adaptivity 0} we have:
$$
I=\sum_{(v_i,\theta_i,S_i)\in\theta^3}k_i\times(S_i+Z_i)= k\times(R_2+I_2)+\sum_{(v_i,\theta_i,S_i)\in\theta^4}k_i\times(S_i+Z_i)
$$
We want to prove $I+R_1+R_3\leq J$.  

Starting from the left hand side we have 
$$
\begin{array}{rcl}
I+R_1+R_3&=&
             \sum_{(v_i,\theta_i,S_i)\in\theta^3}(k_i\times(S_i+Z_i)) +R_1+R_3\\
&=&
             k\times(R_2+I_2)+\sum_{(v_i,\theta_i,S_i)\in\theta^4}k_i\times(S_i+Z_i) +R_3+R_1\\
&\leq&
    k\times(R_2+I_2)+Z'+\sum_{(v_i,\theta_i,S_i)\in\theta^1}k_i^1\times(S_i+Z_i)
    +R_1\\
&\leq&
    k\times(R_2+I_2)+Z'+Z^1+\sum_{(v_i,\theta_i,S_i)\in\theta}k_i^1\times(S_i+Z_i)\\
&=&
    k\times(R_2+\sum_{(v_i,\theta_i,S_i)\in\theta^2}k_i^2\times(S_i+Z_i))\\
&&+Z'+Z^1+\sum_{(v_i,\theta_i,S_i)\in\theta}k_i^1\times(S_i+Z_i)\\
&\leq&
    k\times(Z^2+\sum_{(v_i,\theta_i,S_i)\in\theta}k_i^2\times(S_i+Z_i))\\
&&+Z'+Z^1+\sum_{(v_i,\theta_i,S_i)\in\theta}k_i^1\times(S_i+Z_i)\\
&=&
    k\times Z^2 +Z'+Z^1+\\
&&\sum_{(v_i,\theta_i,S_i)\in\theta}k\times k_i^2\times(S_i+Z_i)) +\sum_{(v_i,\theta_i,S_i)\in\theta}k_i^1\times(S_i+Z_i)\\
&=&
    k\times Z^2 +Z'+Z^1+\sum_{(v_i,\theta_i,S_i)\in\theta}(k_i^1
    +k\times k_i^2)\times(S_i+Z_i)) \\
&=&J\\
\end{array}
$$
This concludes this case.
     \caseL{Case
       \[
           \inferrule{
    \expr , \env \bigstep{\adapt} \valr , \env_1 \\
    \eop{}(\valr\env_1) = \valr'\\
    FV(\valr')=\emptyset
  }{
    \eop(\expr), \env \bigstep{\adapt +1} \valr',  \env_1
  }~\textsf{delta}
       \]
     }
   By assumption, the closure $(\eop(\expr) , \env)$ is
   typable with type $\tau$ and adaptivity $J$.  
Let us assume without
   loss of generality that
   $\env=[x_1 \to (\valr_1 , \env_1 ,
   S_1 ) , \ldots, x_n \to (\valr_n, \env_n, S_n )]$.  By
   Definition~\ref{def:typable} we have that there exist $Z$ and 
   $\bang{k_i} \type_i$ for $(1\leq i\leq n)$ such that:
     \begin{equation}
\label{fact:delta}
       x_1 : \bang{k_1} \type_1, \ldots, x_n:\bang{k_n} \type_n
\tvdash{Z} \eop(\expr) : \type 
\end{equation}
    Moreover, we have that each closure $ (\valr_i, \env_i)\in\theta $ is
    typable with type $\type_i$ and adaptivity $Z_i$, and that 
$$J = Z + \sum_{(v_i,\theta_i,S_i)\in\theta} k_i \times (S_i
  +Z_i).$$
By inversion on Fact~\ref{fact:delta} we have that $Z=Z'+1$ for some
$Z'$, that $\type=\tbase$, that $k_i= k_i'+1$ for $(1\leq i\leq n)$,
and that:
     \begin{equation}
\label{fact:delta}
       x_1 : \bang{k_1'} \type_1, \ldots, x_n:\bang{k_n'} \type_n
\tvdash{Z'} \expr : \tbase.
\end{equation}
Hence, it is easy to see that the closure
$(\expr, \env)$
is typable with type $\tbase$ and adaptivity 
$$Z' + \sum_{(v_i,\theta_i,S_i)\in\theta} k_i' \times (S_i
  +Z_i)$$
By applying the induction hypothesis we have that also 
the closure 
$(v, \env')$ is typable with type $\tbase$ and adaptivity $I'$ such
that:
$$
I'+R\leq Z' + \sum_{(v_i,\theta_i,S_i)\in\theta} k_i' \times (S_i
  +Z_i)
$$
From this and the fact that $\vdash_0 v' :\tbase$, we have:
$$
I'+R+1\leq Z'+1 + \sum_{(v_i,\theta_i,S_i)\in\theta} (k_i'+1) \times (S_i
  +Z_i)
$$
This councludes this case. 
   \end{proof}  

\section{Some examples}
Let us assume $\theta=[x\mapsto (\lambda u.\lambda w.\delta(u)+\delta(w),[\,],0)
      ,y:\mapsto (v,[\,],2) ]$. We have
$$
\inferrule
{
  \inferrule
  {
    \inferrule
    { 
      \empty
    }
    {
      \theta, x\bigstep{0} \lambda u.\lambda
      w.\delta(u)+\delta(w),[\ ]
    }
    \\
    \inferrule
    { 
      \empty
    }
    {
      \theta, y\bigstep{2} v, [\ ]  
    }
    \\
    \inferrule
    { 
      \empty
    }
    {
      [r\mapsto (v,[\ ],2) ], \lambda
      w.\delta(r)+\delta(w)\bigstep{0} \lambda
      w.\delta(r)+\delta(w), [r\mapsto (v,[\ ],2) ]
    }
  }
  {
    \theta, x\, y \bigstep{0} \lambda
      w.\delta(r)+\delta(w), [r\mapsto (v,[\ ],2) ]
    }
    \\
    \inferrule
    { 
      \empty
    }
    {
      \theta, y\bigstep{2} v, [\ ]  
    }
    \\
    \inferrule
    { 
     \inferrule
     {
[r\mapsto (v,[\ ],2),s\mapsto (v,[\ ],2)],
      r\bigstep{2} 
      v, [r\mapsto (v,[\ ],2),s\mapsto (v,[\ ],2)]
     }
     {
       [r\mapsto (v,[\ ],2),s\mapsto (v,[\ ],2)],
       \delta(r)\bigstep{2} 
       v_r, [r\mapsto (v,[\ ],2),s\mapsto (v,[\ ],2)]
     }
     \\
     \inferrule
     {
       [r\mapsto (v,[\ ],2),s\mapsto (v,[\ ],2)],
       r\bigstep{2} 
       v, [r\mapsto (v,[\ ],2),s\mapsto (v,[\ ],2)]
     }
     {
       [r\mapsto (v,[\ ],2),s\mapsto (v,[\ ],2)],
       \delta(s)\bigstep{2} 
       v_s, [r\mapsto (v,[\ ],2),s\mapsto (v,[\ ],2)]
     }
     \\ 
     v_r+v_s=v'
    }
    {
      [r\mapsto (v,[\ ],2),s\mapsto (v,[\ ],2)],
      \delta(r)+\delta(s)\bigstep{4} 
     v', [r\mapsto (v,[\ ],2),s\mapsto (v,[\ ],2)]
    }
}
{
 \theta, x\, y\, y\bigstep{4} v', [r\mapsto (v,[\ ],2),s\mapsto (v,[\ ],2)]
}
$$
