\begin{proof}
  By induction on the typing derivation.\\

  \caseL{
    Case $
      \inferrule{
    }{
      \ictx \tctx , x: \bang{1} \type \tvdash{0} x: \type
    }~\textbf{Ax}
    $
  }

  assume $ \tvdash{\nnatA} (\valr, \env') :  \type$ and $ \tvdash{\nnatA_i} (\valr_i,
  \env_i) :  \type_i  $,
 

  assume $\env =  [x \to (\valr, \env', R)] \uplus [ x_1 \to (\valr_1,
  \env_1, R_1), \ldots,   x_i \to (\valr_i,
  \env_i, R_i)]   $.

  So $\phi = [x \to (1, \adapt, \nnatA) ] \uplus [ x_1 \to (\idx_1,
  \adapt_1, \nnatA_1), \ldots,   x_i \to (\idx_i,  \adapt_i, \nnatA_i)] $

  $F\big(x, \phi \big) = 1 \times (\adapt + \nnatA)  $.

  TS:$\tvdash{0 +1 \times (\adapt+ \nnatA ) } ( x,   \env  ) : \type $.

   
  
  We conclude from the configuratio rule C-Ax.
  
  \[ \inferrule{
     \env ( x ) = (\valr, \env', R)
      \\
      \tvdash{\nnatA} ( \valr, \env') : \type
    }{
     \tvdash{\adapt+\nnatA}   ( x, \env):  \type
    }~\textbf{C-Ax}
  \]

  \caseL{
    Case $
       \inferrule{
      \ictx \Gamma, x: \ltype
      \tvdash{\nnatA }
      \expr: \type
    }{
      \ictx \Gamma \tvdash{0} \lambda x. \expr : \ltype
      \lto{\nnatA} \type
    }~\textbf{lambda}
    $
  }

  let $\Gamma =x_1: \bang{k_1} \type_1 , \ldots,  x_i : \bang{k_i} \type_i$ and  $\ltype = \bang{k} \type_1$.

  Assume $\tvdash{\nnatA'}  (\valr', \env')  :  \type_1 ~(1)$ and $
  \tvdash{\nnatA_i} (\valr_i, \env_i) :  \type_i  $.

Assume  $ \env =  [x_1 \to (\valr_1, \env_1, \adapt_1), \ldots,   x_i \to (\valr_i, \env_i, \adapt_i)]  $.

So $\phi =  [ x_1 \to (\idx_1,
  \adapt_1, \nnatA_1), \ldots,   x_i \to (\idx_i,  \adapt_i, \nnatA_i)] $

  TS: $ \tvdash{0 + F(\lambda x. \expr,  \phi )  }   (\lambda
  x.\expr,  \env) :  \bang{\idx} \type_1  \lto{\nnatA} \type_2 $. 

  Let $S = \sum_{x_i \in \fv{\lambda x. \expr} } \idx_i \times
  (\adapt_i + \nnatA_i)    $ .

  From assumption $(1)$, we know :  $\tvdash{\nnatA' } ( \valr', \env) : \type_1~(\star)$.

  Take a fresh variable x', doing alpha renaming on the premise, pick
  $\adapt'$ so that $\env' = [x' \to (\valr', \env', \adapt' )] \uplus
  \env$ and $\phi'= [x' \to (\idx, \adapt', \nnatA')] \uplus \phi$.
  
  By induction hypothesis on the premise, we know: $\tvdash{ \nnatA+
 F(\expr[x'/x], \phi' ) }  ( \expr[x'/x],  [x' \to (\valr', \env', \adapt')] \uplus \env
) : \type~(\diamond) $.

 $F(\expr[x'/x], \phi' )  = \sum_{x_i \in \fv{\lambda x. \expr} } \idx_i
 \times (\adapt_i +\nnatA_i)  + \idx
 \times (\adapt'+\nnatA')  =  S + \idx \times (\adapt'+ \nnatA' )$.


 We can conclude the following by the configuration rule. 
    
  
  \[
       \inferrule{
      \tvdash{\nnatA'} ( \valr', \theta') : \type_1 ~(\star)
      \\
      \fresh\eapp  x'
      \\
      \tvdash{ S+  \idx \times (\adapt'+\nnatA') +\nnatA }
     ( \expr[x'/x], \env[x' \to (\valr', \env', \adapt')]      ) :
     \type~(\diamond)
    }{
     \tvdash{S} (  \lambda x. \expr, \env )  : \bang{\idx} \type_1
      \lto{\nnatA} \type
    }~\textbf{C-lambda}
  \]


  \caseL{Case
    $
        \inferrule{
      \ictx \Gamma_1  \tvdash{\nnatA_1} \expr_1:  \bang{\idx} \type_1
      \lto{\nnatA} \type_2      \\
      \ictx \Gamma_2 \tvdash{\nnatA_2} \expr_2: \type_1 
    }{
      \ictx   \Gamma_1 + \idx \times \Gamma_2  \tvdash{    \nnatA_1 +
        \idx \times \nnatA_2 + \nnatA    } \expr_1 \eapp \expr_2 : \type_2
    }~\textbf{app}
    $
  }
  
  Let us assume $\Gamma_1 = x_i : \bang{k_i} \type_i $ and $\Gamma_2 = x_i' : \bang{k_i'} \type_i'$,($\Gamma_1$ and $\Gamma_2$ may overleap.).
  
  Forall the variables $x_i''$ in $\dom (\Gamma_1 + k \times \Gamma_2
  )$, we assume $ (\Gamma_1 + k \times
  \Gamma_2 )(x_i'') = \bang{k_i''} \type_i'' $ so that
  $ \tvdash{\nnatA_i''}  (\valr_i'', \env_i'')  : \type_i'' $

  assume $\env = [x_1'' \to (\valr_1'', \env_1'', \adapt_1''), \ldots,
  x_i'' \to (\valr_i'', \env_i'', \adapt_i'')]$.

  So $\phi =  [x_1'' \to (\idx_1'', \adapt_1'', \nnatA_1''), \ldots,
  x_i'' \to (\idx_i'', \adapt_i'', \nnatA_i'')]$

  TS: $ \tvdash{\nnatA_1 + \idx \times \nnatA_2 + \nnatA   +
    F(\expr_1 \eapp \expr_2, \phi ) }   (\expr_1 \eapp \expr_2 , \env)
  : \type_2 $.\\

  let $\env_1 = \{  [x_i'' \to (\valr_i'', \env_i'', R_i'') ]   |     x_i'' \in \dom(\Gamma_1)  \}   $.

  let $\env_2 = \{  [x_i'' \to (\valr_i'', \env_i'', R_i'') ]   |
  x_i'' \in \dom(\Gamma_2)  \}   $.

  We know  $ \dom(\env) = \dom(\env_1) \uplus \dom(\env_2) \implies   \env = \env_1 \uplus \env_2 $

  We set $\phi_1 =\{  [x_i \to (\idx_i'', \adapt_i'', \nnatA_i'')] |
  x_i'' \in \dom(\Gamma_1)  \} $. and $\phi_2 =\{  [x_i \to (\idx_i'', \adapt_i'', \nnatA_i'')] |    x_i'' \in \dom(\Gamma_2)  \} $
  
  By induction hypothesis on the first premise, we have:
  $ \tvdash{ \nnatA_1 + F(\expr_1, \phi_1) } (\expr_1, \env_1) : \bang{\idx} \type_1 \lto{\nnatA} \type_2 ~(\star)$.

  By induction hypothesis on the second premise, we have:
  $ \tvdash{ \nnatA_2 + F(\expr_2, \phi_2 )  } (\expr_2, \env_2) : \type_1 $ .

 From the definition, we know: $ F(\expr_1, \phi_1) = F (\expr_1, \phi) $ and $ F(\expr_2, \phi_2) = F (\expr_2, \phi) $ .
  
  From the configuration rule C-app, we get:

  
  \[
 \inferrule{
       \tvdash{\nnatA_1 + F(\expr_1, \env_1, \Gamma_1) } ( \expr_1, \env_1) :  \bang{\idx} \type_1
      \lto{\nnatA} \type_2    ~(\star)  \\
      \tvdash{\nnatA_2 +  F(\expr_2, \env_2, \Gamma_2)} ( \expr_2, \env_2 ): \type_1 ~(\diamond)
        }{
       \tvdash{    \nnatA_1 + F(\expr_1, \env_1, \Gamma_1) + \idx
         \times (\nnatA_2 +  F(\expr_2, \env_2, \Gamma_2)) + \nnatA
       } (  \expr_1 \eapp \expr_2, \env_1 \uplus \env_2   ) : \type_2 ~(\clubsuit)
    }~\textbf{C-app} 
  \]

  Because $ F(\expr_1,\phi_1)  + \idx \times F(\expr_2,
  \phi_2 ) \leq F(\expr_1 \eapp \expr_2,  \phi) $, so we conclude :$  \nnatA_1 + F(\expr_1,\phi_1) + \idx \times
  (\nnatA_2 +  F(\expr_2, \phi_2)) + \nnatA  \leq \nnatA_1 + \idx
  \times \nnatA_2 + \nnatA   +   F(\expr_1 \eapp \expr_2, \phi )  $ .

  The TS can be shown using Lemma~\ref{mono} on the $\clubsuit$.
  
  
 \end{proof} 
