%%%%%%%%%%%%%%%%%%%%%%%%%%%%%%%%%%%%%%%%%%%%%%%%%%%%%%%%%%%%%%%%%%%%%%%%%%%%%%%%%%%%%%%%%%%%%%%%%%%%%%%%%%
%Proof of old Fundamental Theorem 
%%%%%%%%%%%%%%%%%%%%%%%%%%%%%%%%%%%%%%%%%%%%%%%%%%%%%%%%%%%%%%%%%%%%%%%%%%%%%%%%%%%%%%%%%%%%%%%%%%%%%%%%%%
% \noindent {\bf case}

% \[
%    \inferrule*[right = PAIR]{
%       \Gamma; \dmap_1 \tvdash{\nnatA_1} \expr_1: \type_1 ~ (1) 
%    		\\
%       \Gamma; \dmap_2 \tvdash{\nnatA_2} \expr_2: \type_2 ~ (2)
%       	\\\\
%       \dmap' = \max(\dmap_1,\dmap_2) 
%       	\\
%       \nnatA' = \max(\nnatA_1,\nnatA_2)
%     }{
%       \Gamma; \dmap' \tvdash{\nnatA'} (\expr_1, \expr_2): \type_1 \times \type_2
%     }
% \]
% Assume $(\stepiA, \env) \in \lrv{\Gamma}$, 
% to show: $(\stepiA, (\env, (\expr_1, \expr_2))) \in \lre{\dmap'}{\nnatA'}{\type_1 \times \type_2}$.\\
% %
% By inversion, STS: $\forall \eapp  \valr, \tr, j.$ 
% $(\env, (\expr_1, \expr_2) \bigstep \valr, \eapp  \tr) \land (\size{\tr} = j) \land (j \leq \stepiA)$\\
% %
% $\Rightarrow (\adap(\tr) < \nnatA') \land (\forall x \in \mbox{Vars}. \ddep{x}(\tr) \leq \dmap'(x)) \land ((\stepiA - j, \valr) \in \lrv{\type_1 \times \type_2})$.\\
% %
% By induction hypothesis on $(1)$, we have $(\stepiA, \expr_1) \in \lre{\dmap_1}{\nnatA_1}{\type_1}$.\\
% %
% By inversion, pick any $\valr_1,  \tr_1, j_1$ s.t.,
% $(\env, \expr_1 \bigstep \valr_1, \tr_1) ~ (3) 
% \land (\size{\tr_1} = j_1) 
% \land (j_1 < \stepiA) $,\\
% %
% we have: \\
% $(\adap(\tr_1) \leq \nnatA_1) ~ (4)$ 
% $\land \forall x, \ddep{x}(\tr_1) \leq \dmap_1(x) ~ (5)$ 
% $\land (\stepiA - j_1, \valr_1) \in \lrv{\type_1} ~ (6) $.\\
% %
% By induction hypothesis on $(2)$ and the assumption $(\stepiA - j_1,
% \env) \in \lrv{\Gamma}$ from Lemma~\ref{lem:downward}, we have $(\stepiA - j_1, \expr_2) \in \lre{\dmap_2}{\nnatA_2}{\type_2}$.\\
% %
% By inversion, pick $\valr_2,  \tr_2ï¼Œj_2 $ s.t., $ (\env, \expr_2
% \bigstep \valr_2, \tr_2) ~ (7) \land (\size{\tr_2} = j_2) \land j_2 < \stepiA-j_1 $,\\
% %
% we have:\\
% $\adap(\tr_2) \leq \nnatA_2 ~ (8)$
% $\land \forall x\in \mbox{Vars}. \ddep{x}(\tr_2) \leq \dmap_2(x) ~ (9)$
% $\land (\stepiA- j_1- j_2, \valr_2) \in \lrv{\type_2} ~ (10)$.\\
% %
% By E-Pair rule, we have:\\
% \[
% \inferrule*[right = E-Pair]
% {\env, \expr_1 \bigstep \valr_1, \tr_1 ~ (3)  \and \env, \expr_2
% \bigstep \valr_2, \tr_2 ~ (7) }
% {\env, (\expr_1, \expr_2) \bigstep (\valr_1, \valr_2), (\tr_1, \tr_2)}
% \]
% Pick $\valr = (\valr_1, \valr_2), \tr = (\tr_1, \tr_2), j = |(\tr_1, \tr_2)| = j_1 + j_2$, s.t. $\env, (\expr_1, \expr_2) \bigstep \valr, \tr \land \size{\tr} = j \land j \leq \stepiA$.\\
% %
% STS:\\
% 1. $\adap(\tr) = \adap(\tr_1, \tr_2) < \nnatA' = \max(\nnatA_1, \nnatA_2)$, which is proved by $(4), (8)$.\\
% %
% 2. $\forall x \in \mbox{Vars}. \ddep{x}(\tr_1, \tr_2) = \max(\ddep{x}(\tr_1), \ddep{x}(\tr_2)) \leq \dmap'(x) = \max(\dmap_1(x), \dmap_2(x))$, which is proved by $(5),(9)$.\\
% %
% 3. $(\stepiA - (j_1 + j_2), (\valr_1, \valr_2)) \in \lrv{\type_1
%   \times \type_2}$, which is proved by $(10)
% $ and applying Lemma~\ref{lem:downward} on $(6)$.\\


% \noindent {\bf case}
% \[
%     \inferrule*[right = FIX]{
%       \Gamma, f: (\tarr{\type_1}{\type_2}{\nnatbiA}{\dmap}{\nnatA}), x: \type_1;
%       \dmap[f: \infty, x: \nnatbiA]
%       \tvdash{\nnatA}
%       \expr: \type_2
%        ~ (\triangle)
%     }{
%       \Gamma; \dmap' \tvdash{\nnatA'} \efix f(x).\expr: (\tarr{\type_1}{\type_2}{\nnatbiA}{\dmap}{\nnatA})
%     }
% \]
% Assume: $(\stepiA, \env) \in \lrv{\tr}$. TS: $(\stepiA, (\env, \efix f(x). \expr)) \in \lre{\dmap'}{\nnatA}{\type}$.\\
% %
% By inversion, STS: $\forall \valr, \tr, j.$
% $(\env, \efix f(x). \expr \bigstep \valr, \tr) \land (\size{\tr} = j) \land (j \leq \stepiA)$
% $ \Rightarrow (\adap(\tr) \leq \nnatA') \land (\forall x \in \mbox{Vars}. \ddep{x}(\tr) \leq \dmap'(x)) \land ((\stepiA - j), \valr) \in \lrv{(\tarr{\type_1}{\type_2}{\nnatbiA}{\dmap}{\nnatA})}$.\\
% %
% By E-FIX, let $\valr = (\efix f(x). \expr, \env)$, we know:\\
% $(\env, \efix f(x). \expr) \bigstep ((\efix f(x). \expr, \env), \efix f(x). \expr)~(1) $;\\
% $|\efix f(x). \expr|= j \land j < \stepiA ~(2).$\\
% %
% Suppose $(1), (2)$, STS: $ (\adap(\efix f(x). \expr) = 0 \leq \nnatA')
% \land (\forall x \in \mbox{Vars}. \ddep{x}(\efix f(x). \expr) = \bot \leq \dmap'(x)) \land ((\stepiA -j), (\efix f(x). \expr, \env)) \in \lrv{(\tarr{\type_1}{\type_2}{\nnatbiA}{\dmap}{\nnatA})}$.\\
% %
% The first two goals are proved , we prove the third proposition
% $((\stepiA -j), (\efix f(x). \expr, \env)) \in
% \lrv{(\tarr{\type_1}{\type_2}{\nnatbiA}{\dmap}{\nnatA})}$. To prove
% this,  we first prove on general theorem: \\
% set $\stepiA - j = \stepiA'$, $\forall m \leq \stepiA', (m, (\efix f(x). \expr, \env)) \in \lrv{(\tarr{\type_1}{\type_2}{\nnatbiA}{\dmap}{\nnatA})}$.\\
% %
% Induction on $m$:

% {\bf Subcase 1:} $m = 0$,

% 	TS: $\forall j' < 0$, $(j', \env[\dots] \expr) \in \lre{\nnatA}{\dmap[\dots]}{(\tarr{\type_1}{\type_2}{\nnatbiA}{\dmap}{\nnatA})}$,
	
% 	it is obviously true because $j' < 0 \notin \mathbb{N}$.

% {\bf Subcase 2:} $m = m' + 1 \leq \stepiA'$, 

% 	TS: $ (m, (\efix f(x). \expr, \env)) \in \lrv{(\tarr{\type_1}{\type_2}{\nnatbiA}{\dmap}{\nnatA})}$.

% 	Pick $\forall j' < m' + 1$, $\forall (j', \valr_m) \in \lrv{\type_1}$,
	
% 	STS: $(j', (\env[x \mapsto \valr_m, f \mapsto (\efix f(x).\expr, \env)], \expr)) \in \lre{\dmap[x: \nnatbiA, f: \infty]}{\nnatA}{\type_2} ~ (\star)$.
	
% 	By sub ih, we have:
% 	$(m', (\efix f(x). \expr, \env)) \in \lrv{(\tarr{\type_1}{\type_2}{\nnatbiA}{\dmap}{\nnatA})} ~ (a)$.

% 	Pick $\env' = \env[x \mapsto \valr_m, f \mapsto (\efix f(x).\expr, \env)]$,
	
% 	we know: $(j', \env') \in \lrv{\Gamma,
%           f:(\tarr{\type_1}{\type_2}{\nnatbiA}{\dmap}{\nnatA}),  x:
%           \type_1} ~ (\diamond)$ proved from the following premises:\\ 
	
% 	1. $ (\stepiA, \env) \in \lrv{\Gamma}$, applying Lemma~\ref{lem:downward} on assumption, we get: $(j', \env) \in \lrv{\Gamma}$.
	
% 	2. $(j', \valr_m) \in \lrv{\type}$, from the assumption.
	
% 	3. $(j', (\efix f(x). \expr, \env)) \in \lrv{(\tarr{\type_1}{\type_2}{\nnatbiA}{\dmap}{\nnatA})}$ from $(a)$.\\
% %
% From above, $\star$ is proved by induction hypothesis on $\diamond$ and $\triangle$.\\
% %


% \noindent {\bf case}
% \[
%     \inferrule*[right = APP]
%     {
%       \Gamma; \dmap_1 \tvdash{\nnatA_1} \expr_1: (\tarr{\type_1}{\type_2}{\nnatbiA}{\dmap}{\nnatA})~(\star) \\
%       \Gamma; \dmap_2 \tvdash{\nnatA_2} \expr_2: \type_1 ~(\diamond)\\\\
%       \nnatA' = \nnatA_1 + \max(\nnatA, \nnatA_2 + \nnatbiA) \\
%       \dmap' = \max(\dmap_1, \nnatA_1 + \max(\dmap, \dmap_2 + \nnatbiA))
%     }{
%       \Gamma; \dmap' \tvdash{\nnatA'} \expr_1 \eapp \expr_2 : \type_2
%     }
% \]
% %
% Assume $(\stepiA, \env) \in \lrv{\Gamma} ~ (\square)$, TS: $(\stepiA, (\env, \expr_1 \eapp \expr_2)) \in \lre{\nnatA'}{\dmap'}{\type_2}$.\\
% %
% By inversion, pick any $\valr, \tr, j$ s.t. $((\env, \expr_1 \eapp \expr_2) \bigstep (\valr, \tr)) \land (\size{\tr} = j) \land (j \leq \stepiA) $.\\
% %
% STS: $(\adap(\tr) \leq \nnatA') \land (\forall x \in \mbox{Vars}. \ddep{x}(\tr) \leq \dmap'(x)) \land (((\stepiA - j), \valr) \in \lrv{\type_2})$.\\
% %
% By induction hypothesis on $\star$ and $\square$, we get: $(\stepiA, (\env, \expr_1)) \in \lre{\dmap_1}{\nnatA_1}{\tarr{\type_1}{\type_2}{\nnatbiA}{\dmap}{\nnatA}} ~(1) $.\\
% %
% Inversion on $(1)$, we get:\\
% %
% Pick any $\valr_1, \tr_1, j_1$, s.t. $((\env, \expr_1) \bigstep (\valr_1, \tr_1)) ~(a) \land (\size{\tr_1} = j_1) \land (j_1 < \stepiA)$, \\
% %
% we know: $(\adap(\tr_1) \leq \nnatA_1)~(2) \land (\forall x \in \mbox{Vars}. \ddep{x}(\tr_1) \leq \dmap_1(x))~(3) \land ((\stepiA - j_1), \valr_1) \in \lrv{\tarr{\type_1}{\type_2}{\nnatbiA}{\dmap}{\nnatA}} ~ (4)$\\
% %
% we have: $\valr_1$ is a function.
% %
% Let $\valr_1 = (\efix f(x). \expr, \env') ~(b)$ s.t. $\tr_1= \efix f(x). \expr$\\
% By inversion on $(4)$, we have $\forall j' < (\stepiA - j_1). \forall (j', \valr') \in \lrv{\type_1}. (j', (\env'[x \mapsto \valr', f \mapsto (\efix f(x).\expr, \env')], \expr)) \in \lre{\dmap[x : \nnatbiA, f: \infty]}{\nnatA}{\type_2} ~ (5)$.\\ 
% %
% By induction hypothesis on $\diamond$ and $\square$, we get:
% %
% $(\stepiA, (\env, \expr_2)) \in \lre{\dmap_2}{\nnatA_2}{\type_1} ~(6)$.\\
% %
% Inversion on $(6)$, we get:\\
% %
% Pick any $\valr_2, \tr_2, j_2$, s.t. $((\env, \expr_2) \bigstep (\valr_2, \tr_2))~(c) \land (\size{\tr_2} = j_2) \land (j_2 \leq \stepiA)$,\\
% %
% we know: $(\adap(\tr_2) \leq \nnatA_2)~(7) \land (\forall x \in \mbox{Vars}. \ddep{x}(\tr_2) \leq \dmap_2(x))~(8) \land ((\stepiA - j_2), \valr_2) \in \lrv{\type_1} ~ (9)$\\
% %
% Apply Lemma~\ref{lem:downward} on $(9)$, we have $((\stepiA - j_2 - j_1-1), \valr_2) \in \lrv{\type_1}$\\
% %
% Pick $j' = \stepiA - j_1 - j_2 - 1, \valr' = \valr_2$, we have: $(\stepiA - j_1 - j_2-1, (\env'[x \mapsto \valr_2, f \mapsto \valr_1], \expr)) \in \lre{\dmap[x : \nnatbiA, f: \infty]}{\nnatA}{\type_2} ~ (10)$ from $(5)$.\\
% %
% Inversion on $(10)$, let $\env'' = \env'[x \mapsto \valr_2, f \mapsto \valr_1]$, pick any $\valr'', \tr'', j''$, s.t. $((\env'', \expr) \bigstep (\valr'', \tr''))~(d) \land (\size{\tr''} = j'') \land (j'' \leq \stepiA - j_1 - j_2-1)$, we have:\\
% %
% $\adap(\tr'') \leq n ~(11)  \land (\forall x \in \ddep{x}(\tr'')\leq
% \dmap[x : \nnatbiA, f: \infty](x)) ~(12) \land (\stepiA - j_1 - j_2 - j''-1, \valr'') \in \lrv{\type_2}~(13)$.\\
% %
% Apply E-APP rule on $(a) (b) (c) (d)$ we have:
% \[
%   \inferrule{
%     \env, \expr_1 \bigstep \valr_1, \tr_1 ~ (a) \\
%     \valr_1 = (\efix f(x).\expr, \env')~(b) \\\\
%     \env, \expr_2 \bigstep \valr_2, \tr_2 ~ (c) \\
%     \env'[f \mapsto \valr_1, x \mapsto \valr_2], \expr \bigstep \valr'', \tr'' ~(d)
%   }{
%     \env, \expr_1 \eapp \expr_2 \bigstep \valr'', \trapp{\tr_1}{\tr_2}{f}{x}{\tr''}
%   }
% \]
% Pick $\valr = \valr'', j = j_1 + j_2 + j'' + 1, \tr =
% \trapp{\tr_1}{\tr_2}{f}{x}{\tr''}$ s.t. $ \env, \expr_1 \eapp \expr_2
% \bigstep \valr, \tr  \land |tr| = j \land j \leq k $.  \\
% Suffice to show the follwing three:\\
% %
% 1. $\adap(\tr) = \adap(\trapp{\tr_1}{\tr_2}{f}{x}{\tr''}) =
% \adap(\tr_1) + \max(\adap(\tr''), \adap(\tr_2) + \ddep{x}(\tr'')) \leq
% \nnatA_1 + \max(\nnatA, \nnatA_2 + \nnatbiA) = \nnatA'$ proved by $(2),(7),(11),(12)$.\\
% %
% 2. $\forall y \in \mbox{Vars}. \ddep{y}(\tr) = \max(\ddep{y}(\tr_1), \adap(\tr_1) +
% \max(\ddep{y}(\tr''), \ddep{y}(\tr_2) + \ddep{x}(\tr''))) \leq
% \max(\dmap_1, \nnatA_1 + \max(\dmap, \dmap_2 + \nnatbiA)) = \dmap'(y)$
% proved by $(2),(3),(8),(12)$. \\
% %
% 3. $(\stepiA - j, \valr) = (\stepiA - j_1 - j_2 - j''-1, \valr'') \in
% \lrv{\type_2}$ proved by $(13)$.\\
% %


% \noindent {\bf case}
% \[
%     \inferrule*[right = IF]{
%       \Gamma; \dmap_1 \tvdash{\nnatA_1} \expr_1: \tbool ~ (\star) \\
%       \Gamma; \dmap \tvdash{\nnatA} \expr_2: \type ~(\diamond) \\
%       \Gamma; \dmap \tvdash{\nnatA} \expr_3: \type ~(\triangle) \\\\
%       \nnatA' = \nnatA_1 + \nnatA \\
%       \dmap' = \max(\dmap_1, \nnatA_1 + \dmap)
%     }{
%       \Gamma; \dmap' \tvdash{\nnatA'} \eif(\expr_1, \expr_2, \expr_3):  \type
%     }
% \]
% Assume $(\stepiA, \env) \in \lrv{\Gamma}$, TS: $(\stepiA, (\env, \eif(\expr_1, \expr_2, \expr_3))) \in \lre{\dmap'}{\nnatA'}{\type}$.\\
% %
% Inversion on it, $\forall \valr, \tr, j$ $(\env, \eif(\expr_1, \expr_2, \expr_3) \bigstep \valr, \tr) \land (\size{\tr} = j) \land (j \leq \stepiA)$\\
% %
% STS: $(\adap(\tr) \leq \nnatA') \land (\forall x \in \mbox{Vars}. \ddep{x}(\tr) \leq \dmap'(x)) \land ((\stepiA - j, \valr) \in \lrv{\type})$.\\
% %
% By induction hypothesis on $\star$ and $(\stepiA-1, \env) \in
% \lrv{\Gamma}$ by  Lemma~\ref{lem:downward}, we get: $(\stepiA-1, (\env, \expr_1)) \in \lre{\dmap_1}{\nnatA_1}{\tbool} ~(1)$.\\
% %
% Inversion on $(1)$, pick $ \valr_1, \tr_1, j_1. (\env, \expr_1 \bigstep \valr_1, \tr_1) ~ (a) \land (\size{\tr_1} = j_1) \land (j_1 \leq \stepiA-1)$,\\
% %
% we know: $(\adap(\tr_1) \leq \nnatA_1)~(4) \land (\forall x. \in
% \ddep{x}(\tr_1) \leq \dmap_1(x)) ~(5) \land ((\stepiA -1- j_1, \valr_1) \in \lrv{\tbool})$\\
% %
% By induction hypothesis on $\diamond$ and $(\stepiA-1-j_1, \env) \in
% \lrv{\Gamma}$ by Lemma~\ref{lem:downward} on the assumption, we get: $(\stepiA-1-j_1, (\env, \expr_2)) \in \lre{\dmap}{\nnatA}{\type} ~(2)$\\
% %
% By induction hypothesis on $\triangle$ and $(\stepiA-1-j_1, \env) \in
% \lrv{\Gamma}$ , we get: $(\stepiA-1-j_1, (\env, \expr_3)) \in \lre{\dmap}{\nnatA}{\type} ~(3)$\\
% %
% Induction on $\valr_1$, we have two following subcases:

% {\bf Subcase1:} $\valr_1 = \etrue$, \\
% %
% inversion on $(2)$, pick any $\valr_2, \tr_2, j_2. (\env, \expr_2 \bigstep \valr_2, \tr_2) ~ (b) \land (\size{\tr_2} = j_2) \land (j_2 \leq \stepiA-1-j_1)$,\\
% %
% we know: $(\adap(\tr_2) \leq \nnatA)~(6) \land (\forall x \in \mbox{Vars}. \ddep{x}(\tr_2) \leq \dmap(x))~(7) \land ((\stepiA-1 - j_1-j_2, \valr_2) \in \lrv{\type})~(8)$.\\
% %
% Apply E-IFT on $(a) (b)$, we get:
% \[
%   \inferrule{
%     \env, \expr_1 \bigstep \etrue, \tr_1 ~ (a) \\
%     \env, \expr_2 \bigstep \valr_2, \tr_2 ~ (b)
%   }{
%     \env, \eif(\expr_1, \expr_2, \expr_3) \bigstep \valr_2, \trift(\tr_1, \tr_2)
%   }
% \]
% Pick $\valr = \valr_2, \tr = \trift(\tr_1, \tr_2), j =j_1+ j_2+1$ s.t. $
% \env, \eif(\expr_1, \expr_2, \expr_3) \bigstep \valr, \tr \land j =
% |tr| \land j = j_1 + j_2+1 \leq k$.\\
%  STS the following 3 goals:\\
% %
% 1. $\adap(\tr) = \adap(\trift(\tr_1, \tr_2)) = \adap(\tr_1) +
% \adap(\tr_2)) \leq \nnatA_1 + \nnatA = \nnatA'$. proved by $(4),(6)$.\\
% %
% 2. $\forall x \in \mbox{Vars} . \ddep{x}(\tr) = \max(\ddep{x}(\tr_1), \adap(\tr_1) +
% \ddep{x}(\tr_2)) \leq \max(\dmap_1(x), \nnatA_1(x) + \dmap(x)) =
% \dmap'(x)  $ proved by $(5), (7)$.\\
% %
% 3. $(\stepiA - j, \valr) = (\stepiA-1 -j_1- j_2, \valr_2) \in
% \lrv{\type}$ proved by $(8)$.

% {\bf Subcase2:} $\valr_1 = \efalse$\\
% %
% inversion on $(3)$, pick any $\valr_3, \tr_3, j_3. (\env, \expr_3 \bigstep \valr_3, \tr_3) ~ (b) \land (\size{\tr_3} = j_3) \land (j_3 \leq \stepiA-1-j_1)$,\\
% %
% we know: $(\adap(\tr_3) \leq \nnatA) ~(9) \land (\forall x \in
% \mbox{Vars}. \ddep{x}(\tr_3) \leq \dmap(x))~(10) \land ((\stepiA -1-j_1- j_3, \valr_3) \in \lrv{\type})~(11)$.\\
% %
% Apply E-IFT on $(a) (b)$, we get:
% \[
%   \inferrule{
%     \env, \expr_1 \bigstep \etrue, \tr_1 ~ (a) \\
%     \env, \expr_3 \bigstep \valr_3, \tr_3 ~ (b)
%   }{
%     \env, \eif(\expr_1, \expr_2, \expr_3) \bigstep \valr_3, \trift(\tr_1, \tr_3)
%   }
% \]
% Pick $\valr = \valr_3, \tr = \trift(\tr_1, \tr_3), j =j_1+ j_3+1$,  s.t. $
% \env, \eif(\expr_1, \expr_2, \expr_3) \bigstep \valr, \tr \land j =
% |tr| \land j = j_1 + j_3+1 \leq k$.\\
%  STS the following 3 goals:\\
% %
% 1. $\adap(\tr) = \adap(\trift(\tr_1, \tr_3)) = \adap(\tr_1) +
% \adap(\tr_3)) \leq \nnatA_1 + \nnatA = \nnatA'$  proved by $(4),(9)$.\\
% %
% 2. $\forall x \in \mbox{Vars}. \ddep{x}(\tr) = \max(\ddep{x}(\tr_1), \adap(\tr_1) +
% \ddep{x}(\tr_3)) \leq \max(\dmap_1(x), \nnatA_1(x) + \dmap(x)) =
% \dmap'(x) $ proved by $(5),(10)$.\\
% %
% 3. $(\stepiA - j, \valr) = (\stepiA -1 - j_1-j_3, \valr_3) \in
% \lrv{\type} $ proved by $(11)$.\\



% \noindent {\bf case}
% \[
%     \inferrule*[right = FST]{
%       \Gamma; \dmap \tvdash{\nnatA} \expr: \type_1 \times \type_2
%     }{
%       \Gamma; \dmap \tvdash{\nnatA} \eprojl(\expr): \type_1
%     }
% \]
% Assume $(\stepiA, \env) \in \lrv{\Gamma}$, TS: $(\stepiA, (\env, \eprojl(\expr))) \in \lre{\dmap}{\nnatA}{\type_1} $.\\
% %
% Unfold, pick any $ \valr, \tr, j. (\env, \eprojl(\expr)   \bigstep \valr, \tr) \land (\size{\tr} = j) \land (j \leq \stepiA) $,\\
% %
% STS: $ (\adap(\tr) \leq \nnatA) \land (\forall x \in \mbox{Vars}. \ddep{x}(\tr) \leq \dmap(x)) \land (\stepiA - j, \valr) \in \lrv{\type_1} $.\\
% %
% By induction hypothesis, we get: $(\stepiA-1, (\env, \expr)) \in \lre{\dmap}{\nnatA}{\type_1 \times \type_2} ~(1)$.\\
% %
% Inversion on $(1)$, $\forall \valr', \tr', j'. (\env, \expr \bigstep \valr', \tr') \land (\size{\tr'} = j') \land (j' \leq \stepiA-1) $,\\
% %
% We know: $(\adap(\tr') \leq \nnatA) ~ (a) 
% \land (\forall x \in \mbox{Vars}. \ddep{x}(\tr') \leq \dmap(x)) ~ (b)
% \land ((\stepiA -1 - j', \valr') \in \lrv{\type_1 \times \type_2}) ~ (c)$.\\
% %
% Pick any $\valr_1, \valr_2$, $\valr' = (\valr_1, \valr_2)$,
% % Let $\expr = (\expr_1, \expr_2)$, by E-PAIR, we have:\\
% % %
% % $\tr' = (\tr_1, \tr_2), \valr' = (\valr_1, \valr_2), j' = \size{\tr'} = \size{\tr_1} + \size{\tr_2} = j_1 + j_2$.\\
% %
% inversion on $(c)$, we have:\\
% %
% $(\stepiA - j', \valr_1) \in \lrv{\type_1}~(d) \land (\stepiA - j', \valr_2) \in \lrv{\type_2}$.\\
% %
% By E-FST, pick $\valr = \valr_1, j = j'+1, \tr = \trprojl(\tr')$, STS:\\
% %
% 1. $\adap(\tr) = \adap(\trprojl(\tr')) = \adap(\tr') \leq \nnatA$ by $(a)$.\\
% %
% 2. $\forall x .\ddep{x}(\tr) \implies \forall x . \ddep{x}(\tr') \leq \dmap(x)$ by $(b)$.\\
% %
% 3. $(\stepiA - j, \valr) = (\stepiA -1- j', \valr_2) \in
% \lrv{\type_1}$ by $(d)$.
% \\




% \noindent {\bf case}
% \[
%     \inferrule*[right = SND]{
%       \Gamma; \dmap \tvdash{\nnatA} \expr: \type_1 \times \type_2
%     }{
%       \Gamma; \dmap \tvdash{\nnatA} \eprojr(\expr): \type_2
%     }
% \]
% Assume $(\stepiA, \env) \in \lrv{\Gamma}$, TS: $(\stepiA, (\env, \eprojr(\expr))) \in \lre{\dmap}{\nnatA}{\type_2} $.\\
% %
% Unfold, pick any $ \valr, \tr, j. (\env, \eprojr(\expr) \bigstep \valr, \tr) \land (\size{\tr} = j) \land (j \leq \stepiA) $,\\
% %
% STS: $ (\adap(\tr) \leq \nnatA) \land (\forall x \in \mbox{Vars}. \ddep{x}(\tr) \leq \dmap(x)) \land (\stepiA - j, \valr) \in \lrv{\type_1} $.\\
% %
% By induction hypothesis, we get: $(\stepiA-1, (\env, \expr)) \in \lre{\dmap}{\nnatA}{\type_1 \times \type_2} ~(1)$.\\
% %
% Inversion on $(1)$, $\forall \valr', \tr', j'. (\env, \expr \bigstep \valr', \tr') \land (\size{\tr'} = j') \land (j' \leq \stepiA-1) $,\\
% %
% We know: $(\adap(\tr') \leq \nnatA) ~ (a) 
% \land (\forall x \in \ddep{x}(\tr') \leq \dmap(x)) ~ (b)
% \land ((\stepiA -1- j', \valr') \in \lrv{\type_1 \times \type_2}) ~ (c)$.\\
% %
% Pick any $\valr_1, \valr_2$, $\valr' = (\valr_1, \valr_2)$,
% % Let $\expr = (\expr_1, \expr_2)$, by E-PAIR, we have:\\
% % %
% % $\tr' = (\tr_1, \tr_2), \valr' = (\valr_1, \valr_2), j' = \size{\tr'} = \size{\tr_1} + \size{\tr_2} = j_1 + j_2$.\\
% %
% inversion on $(c)$, we have:\\
% %
% $(\stepiA - j', \valr_1) \in \lrv{\type_1}~(d) \land (\stepiA - j', \valr_2) \in \lrv{\type_2}~(e)$.\\
% %
% By E-SND, pick $\valr = \valr_2, j = j'+1, \tr = \trprojr(\tr')$, STS:\\
% %
% 1. $\adap(\tr) = \adap(\trprojr(\tr')) = \adap(\tr') \leq \nnatA$ by $(a)$\\
% %
% 2. $\forall x \in \mbox{Vars} .\ddep{x}(\tr) \implies \forall x . \ddep{x}(\tr') \leq
% \dmap(x)$ proved by $(b)$.\\
% %
% 3. $(\stepiA - j, \valr) = (\stepiA -1 - j', \valr_2) \in \lrv{\type_2}$
% proved by $(e)$.\\


% \noindent {\bf case}
% \[
%     \inferrule*[right = TRUE]{
%     }{
%       \Gamma; \dmap \tvdash{\nnatA} \etrue: \tbool
%     }
% \]
% Assume $ (\stepiA, \env) \in \lrv{\tbool} $, TS: $(\stepiA, (\env, \etrue)) \in \lre{\dmap}{\nnatA}{\tbool}$.\\
% %
% By inversion, STS: $\forall \valr, \tr, j. (\env, \etrue \bigstep \valr, \tr) \land (\size{\tr} = j) \land (j \leq \stepiA) $\\
% $\Rightarrow$ 
% $ (\adap(\tr) \leq \nnatA) ~ (a) 
% \land (\forall x \in \mbox{Vars}. \ddep{x}(\tr) \leq \dmap(x)) ~ (b)
% \land (\stepiA - j, \valr) \in \lrv{\tbool} ~ (c)$\\
% %
% By E-TRUE, let $\valr = \etrue$, $\tr = \etrue$ and $j = \size{\etrue} = 0$.\\
% %
% The following 3 items are proved:\\
% %
% 1. $\adap(\tr) = 0 \leq \nnatA$.\\
% 2. $\forall x \in \mbox{Vars}. \ddep{x}(\etrue) = 0 \leq \dmap(x)$\\
% 3. $(\stepiA - j, \valr) = (\stepiA, \etrue) \in \lrv{\tbool}$.\\



% \noindent {\bf case}
% \[
%     \inferrule*[right = FALSE]{
%     }{
%       \Gamma; \dmap \tvdash{\nnatA} \efalse: \tbool
%     }
% \]
% Assume $ (\stepiA, \env) \in \lrv{\tbool} $, TS: $(\stepiA, (\env, \efalse)) \in \lre{\dmap}{\nnatA}{\tbool}$.\\
% %
% By inversion, STS: $\forall \valr, \tr, j. (\env, \efalse \bigstep \valr, \tr) \land (\size{\tr} = j) \land (j \leq \stepiA) $\\
% $\Rightarrow$ 
% $ (\adap(\tr) \leq \nnatA) ~ (a) 
% \land (\forall x \in  \mbox{Vars}. \ddep{x}(\tr) \leq \dmap(x)) ~ (b)
% \land (\stepiA - j, \valr) \in \lrv{\tbool} ~ (c)$\\
% %
% By E-TRUE, let $\valr = \efalse$, $\tr = \efalse$ and $j = \size{\efalse} = 0$.\\
% %
% The following 3 items are proved:\\
% %
% 1. $\adap(\tr) = 0 \leq \nnatA$.\\
% 2. $\forall x \in \mbox{Vars}. \ddep{x}(\efalse) = 0 \leq \dmap(x)$\\
% 3. $(\stepiA - j, \valr) = (\stepiA, \efalse) \in \lrv{\tbool}$.\\


% \noindent {\bf case}
% \[
%     \inferrule*[right = PRIMITIVE]{
%       \Gamma; \dmap \tvdash{\nnatA} \expr: \tbase ~ (\star) \\
%       \nnatA' = 1 + \nnatA \\
%       \dmap' = 1 + \dmap
%     }{
%       \Gamma; \dmap' \tvdash{\nnatA'} \eop(\expr): \tbool
%     }
% \]
% Assume $(\stepiA, \env) \in \lrv{\Gamma}$, TS: $(\stepiA, (\eop(\expr), \env)) \in \lre{\dmap'}{\nnatA'}{\tbool}$.\\
% %
% Unfold, $\forall \valr, \tr, j. (\env, \eop(\expr) \bigstep \valr, \tr) \land (\size{\tr} = j) \land (j \leq \stepiA)$.\\
% %
% STS: $(\adap(\tr) \leq \nnatA') \land (\forall x \in \mbox{Vars}. \ddep{x}(\tr) \leq \dmap'(x)) \land ((\stepiA - j, \valr) \in \lrv{\tbool})$.\\
% %
% By induction hypothesis on $\star$, we get: $(\stepiA-1, (\expr, \env)) \in \lre{\dmap}{\nnatA}{\tbase} ~ (1)$.\\
% %
% Inversion on $(1)$, pick $\forall \valr', \tr', j'$. s.t. $ (\env, \expr \bigstep \valr', \tr') \land (\size{\tr'} = j') \land (j' \leq \stepiA-1)$.\\
% %
% We know: $(\adap(\tr') \leq \nnatA) ~ (a)
% \land (\forall x \in \ddep{x}(\tr') \leq \dmap(x)) ~ (b)
% \land ((\stepiA -1- j', \valr') \in \lrv{\tbase}) ~ (c)$.\\
% %
% Pick $\valr = \eop(\valr')$, then by E-PRIMITIVE, we have $\env, \eop(\expr) \bigstep \valr, \eop(\tr')$.\\
% %
% Pick $\tr = \eop(\tr'), j = j' + 1$ s.t.  $j \leq k$, STS:\\
% %
% 1. $\adap(\tr) = \adap(\eop(\tr')) = 1 + \adap(\tr') \leq 1 + \nnatA = \nnatA'$ proved by $(a)$\\
% %
% 2. $\forall x \in \mbox{Vars}. \ddep{x}(\tr) = \ddep{x}(\eop(\tr')) = 1 + \ddep{x}(\tr') \leq 1 + \dmap(x) = \dmap'(x)$ proved by $(b)$\\
% %
% 3. $(\stepiA - j, \valr) = (\stepiA - j' - 1, \eop(\valr')) \in \lrv{\tbool} $.\\
% %
% By typing rule PRIMITIVE, we have $\eop(\valr'): \tbool$. $\eop(\valr')$ is either $\etrue$ or $\efalse$. So, we have $(\stepiA - j' - 1, \eop(\valr')) \in \lrv{\tbool}$.\\
% %



% \noindent {\bf case}
% \[    
% 	\inferrule*[right = VAR]{
%       \Gamma(x) = \type \\ 0 \leq \dmap(x) \mbox{ or equiv.\ } \dmap(x) \neq \bot
%     }{
%       \Gamma; \dmap \tvdash{\nnatA} x: \type
%     }
% \]
% Assume $(\stepiA, \env) \in \lrv{\Gamma}$, TS: $(\stepiA, (\env, x)) \in \lre{\dmap}{\nnatA}{\type}$.\\
% %
% By inversion, STS: $\forall \valr, \tr, j. (\env, x \bigstep \valr, \tr) \land (\size{\tr} = j) \land (j \leq \stepiA) $\\
% $\Rightarrow$ 
% $ (\adap(\tr) \leq \nnatA) ~ (a) 
% \land (\forall x \in \mbox{Vars}. \ddep{x}(\tr) \leq \dmap(x)) ~ (b)
% \land (\stepiA - j, \valr) \in \lrv{\type} ~ (c)$\\
% %
% By E-VAR, pick $\valr = \env(x)$, $\tr = x$, $j = \size{x} = 0$, following 3 items are proved:\\
% %
% 1. $(\adap(\tr) = \adap(x) = 0 \leq \nnatA)$\\
% 2. $\forall y \in \ddep{y}(x)$, \\
% $~~ y = x ~~ \ddep{y}(x) = 0 \leq \dmap(x)$\\
% $~~ y \neq x ~~ \ddep{y}(x) = \bot \leq \dmap(y)$\\
% 3. $(\stepiA - j, \valr) = (\stepiA, \env(x)) \in \lrv{\type}$.\\
% $~~$By definition of $(\stepiA, \env) \in \lrv{\Gamma}$, we have: $(\stepiA, \env(x))\in \lrv{\Gamma(x)}$, and $\Gamma(x) = \type$. 


% \noindent {\bf case}
% \[    
%  \inferrule{
%      \dmap \wf{\type} \\
%     }{
%       \Gamma; \dmap \tvdash{\nnatA} \enil: \tlist{\type}
%     }
% \]
% Assume $(\stepiA, \env) \in \lrv{\Gamma}$, TS: $(\stepiA, (\env, \enil)) \in \lre{\dmap}{\nnatA}{\tlist{\type}}$.\\
% %
% By inversion, STS: $\forall \valr, \tr, j. (\env, \enil \bigstep \valr, \tr) \land (\size{\tr} = j) \land (j \leq \stepiA) $\\
% $\Rightarrow$ 
% $ (\adap(\tr) \leq \nnatA) ~ (a) 
% \land (\forall x \in \mbox{Vars}. \ddep{x}(\tr) \leq \dmap(x)) ~ (b)
% \land (\stepiA - j, \valr) \in \lrv{\type} ~ (c)$\\
% %
% By E-NIL, we know : $ v = \enil $ and $ \tr = \trnil$ and $
% \size{\enil} = 0 \leq k$. \\
% STS: 
% %
% 1. $(\adap(\tr) = \adap(\enil) = 0 \leq \nnatA)$, because $\nnatA$ is
% not negative.\\
% 2. $\forall x \in \mbox{Vars}. \ddep{x}(\enil)$, $  \ddep{x}(\enil) = \bot \leq
% \dmap(x)$ proved from the definition of $\bot$. \\
% 3. $(\stepiA - 0, \enil) =  \in \lrv{ \tlist{ \type} }$, proved by
% inversion of the interpretation of $\lrv{ \tlist{ \type} } $.\\

% \noindent{\bf case}
% \[
%   \inferrule{
%    \Gamma; \dmap_1 \tvdash{\nnatA_1} \expr_1 : \type ~(\star) \\
%    \Gamma; \dmap_2 \tvdash{\nnatA_2} \expr_2 : \tlist{\type} ~(\diamond)\\
%    \dmap' = \max(\dmap_1, \dmap_2) \\
%    \nnatA' = \max ( \nnatA_1, \nnatA_2 )
%    }
%    { \Gamma; \dmap' \tvdash{\nnatA'} \econs(\expr_1, \expr_2) :
%      \tlist{\type}  }
% \]

% Assume $(\stepiA, \env) \in \lrv{\Gamma}$, TS: $(\stepiA, (\env,
% \econs(\expr_1 , \expr_2 ) )) \in \lre{\dmap'}{\nnatA'}{\tlist{\type}}$.\\
% %
% By inversion, STS: $\forall \valr, \tr, j. (\env, \econs(e_1,e_2) \bigstep \valr, \tr) \land (\size{\tr} = j) \land (j \leq \stepiA) $\\
% $\Rightarrow$ 
% $ (\adap(\tr) \leq \nnatA')  
% \land (\forall x \in \mbox{Vars}. \ddep{x}(\tr) \leq \dmap'(x)) 
% \land (\stepiA - j, \valr) \in \lrv{\tlist{\type}} $
% %

%   By ih on $(\star)$, we get: $(\stepiA, (\env,
% \expr_1  )) \in \lre{\dmap_1}{\nnatA_1}{\type}~(1)$.\\
% %
% By inversion, we pick $v_1$, $\tr_1$ and $j_1$ s.t. $\env, \expr_1
% \bigstep \valr_1, \tr_1$ and $\size{\tr_1} = j_1$ and $j_1 \leq \stepiA$.\\
% %
% We know : $ (\adap(\tr_1) \leq \nnatA_1) ~ (2) 
% \land (\forall x \in \mbox{Vars}. \ddep{x}(\tr_1) \leq \dmap_1(x)) ~ (3)
% \land (\stepiA - j_1, \valr_1) \in \lrv{\type} ~ (4)$.

%  By ih on $(\diamond)$ and $(\stepiA-j_1, \env) \in \lrv{\Gamma}$ by Lemma~\ref{lem:downward}, we get: $(\stepiA-j_1, (\env,
% \expr_2  )) \in \lre{\dmap_2}{\nnatA_2}{ \tlist{ \type} }~(5)$.\\
% %
% By inversion, we pick $v_2$, $\tr_2$ and $j_2$,  s.t. $\env, \expr_2
% \bigstep \valr_2, \tr_2$ and $\size{\tr_2} = j_2$ and $j_2 \leq
% \stepiA-j_1$.\\
% %
% We know : $ (\adap(\tr_2) \leq \nnatA_2) ~ (6) 
% \land (\forall x \in \mbox{Vars}. \ddep{x}(\tr_2) \leq \dmap_2(x)) ~ (7)
% \land (\stepiA - j_2, \valr_2) \in \lrv{\tlist{\type}} ~ (8)$.
% %
% \[
% \inferrule{
% \env, \expr_1 \bigstep \valr_1, \tr_1 \\
% \env, \expr_2 \bigstep \valr_2, \tr_2
% }
% { \env, \econs (\expr_1, \expr_2)  \bigstep \econs (\valr_1, \valr_2),
%   \trcons(\tr_1, \tr_2)
% }
% \]
% %
% By E-Cons, we set : $\valr = \econs(\valr_1, \valr_2)$ and $\tr =
% \trcons(\tr_1, \tr_2)$ s.t. $j = \size{\tr}= j_1 + j_2 \leq k$.\\
% STS: 
% %
% 1. $(\adap(\tr) = \adap(\trcons(\tr_1, \tr_2)) \leq
% \nnatA')$, by $(2)$ and $(6)$.\\
% 2. $\forall x \in \mbox{Vars}. \ddep{x}(\trcons(\tr_1, \tr_2))
% = \max ( \ddep{x}(\tr_1), \ddep{x}(\tr_2) ) \leq
% \dmap'(x)$ proved by $(3)$ and $(7)$. \\
% 3. $(\stepiA - j_1 -j_2, \econs(\valr_1,\valr_2)  )  \in \lrv{ \tlist{
%     \type} }$, by inversion of the definition of
% $\lrv{\tlist{\type}}$, suffice to show: $(\stepiA-j_1-j_2, \valr_1) \in
%  \lrv{\type}$ proved by Lemma~\ref{lem:downward} on $(4)$, $(\stepiA-j_1-j_2, \valr_2) \in
%  \lrv{ \tlist{\type}} $ proved by $(8)$.\\


% \noindent{\bf case}
% \[
%  \inferrule{
%      \Gamma; \dmap_1 \tvdash{\nnatA_1} \expr_1 : \type_1~(\star) \\
%      \Gamma, x:\type_1 ; \dmap_2[x:q] \tvdash{\nnatA_2} \expr_2 :
%      \type_2 ~(\diamond)\\
%      \dmap' = \max( \dmap_2, \dmap_1 + q ) \\
%      \nnatA' = \max ( \nnatA_2, \nnatA_1 + q )
%    }
%    {  \Gamma; \dmap' \tvdash{\nnatA'}  \elet x = \expr_1 \ein \expr_2 : \type}
% \]
% Assume $(\stepiA, \env) \in \lrv{\Gamma}$, TS: $(\stepiA, (\env,
% \elet x = \expr_1 \ein \expr_2 )) \in \lre{\dmap'}{\nnatA'}{\type}$.\\
% %
% By inversion, STS: $\forall \valr, \tr, j. (\env, \elet x = \expr_1 \ein \expr_2 \bigstep \valr, \tr) \land (\size{\tr} = j) \land (j \leq \stepiA) $\\
% $\Rightarrow$ 
% $ (\adap(\tr) \leq \nnatA')  
% \land (\forall x \in \mbox{Vars}. \ddep{x}(\tr) \leq \dmap'(x)) 
% \land (\stepiA - j, \valr) \in \lrv{\type} $
% %

% By ih on $(\star)$, we get: $(\stepiA, (\env,
% \expr_1  )) \in \lre{\dmap_1}{\nnatA_1}{\type_1}~(1)$.\\
% %
% By inversion, we pick $v_1$, $\tr_1$ and $j_1$ s.t. $\env, \expr_1
% \bigstep \valr_1, \tr_1$ and $\size{\tr_1} = j_1$ and $j_1 \leq \stepiA$.\\
% %
% We know : $ (\adap(\tr_1) \leq \nnatA_1) ~ (2) 
% \land (\forall x \in \mbox{Vars}. \ddep{x}(\tr_1) \leq \dmap_1(x)) ~ (3)
% \land (\stepiA - j_1, \valr_1) \in \lrv{\type_1} ~ (4)$.
% %
% From the assumption  $(\stepiA, \env) \in \lrv{\Gamma}$, by
% Lemma~\ref{lem:downward}, we get : $(\stepiA-j_1, \env) \in
% \lrv{\Gamma}~(5)$. \\
% Set $\env' = \env[x \mapsto \valr_1]$, we know $(\stepiA-j_1, \env')
% \in \lrv{\Gamma,x:\type_1} ~(6) $ by $(4)$ and $(5)$.
% %

% By ih on $(\diamond)$ and $(6)$, we know: $(\stepiA-j_1, (\env',
% \expr_2  )) \in \lre{\dmap_2[x:q]}{\nnatA_2}{\type} ~(7) $.\\
% %
% By inversion $(7)$, we pick $v_2$, $\tr_2$ and $j_2$ s.t. $\env', \expr_2
% \bigstep \valr_2, \tr_2$ and $\size{\tr_2} = j_2$ and $j_2 \leq
% \stepiA - j_1$.\\
% %
% We know:  $ (\adap(\tr_2) \leq \nnatA_2) ~ (8) 
% \land (\forall x \in \mbox{Vars}. \ddep{x}(\tr_2) \leq \dmap_2[x:q](x)) ~ (9)
% \land (\stepiA - j_1 - j_2, \valr_2) \in \lrv{\type} ~ (10)$.
% %
% \[
% \inferrule{
%   \env, \expr_1 \bigstep \valr_1, \tr_1 \\
%   \env[x \mapsto \valr_1] , \expr_2 \bigstep \valr_2, \tr_2
% }
% {\env, \elet x;q = \expr_1 \ein \expr_2 \bigstep \valr_2, \trlet (x,
%   \tr_1, \tr_2) }
% \]
% By E-LET, we know : $\valr = c/valr_2$ and $\tr = \trlet (x,
%   \tr_1, \tr_2)  $. s.t. $j = j_1 +j_2 \leq k$.\\
% %
% STS: 
% %
% 1. $(\adap(\tr) = \adap(\trlet (x,
%   \tr_1, \tr_2) ) \leq
% \nnatA')$, proved by $(2)$ ,$(8)$and $(9)$.\\
% 2. $\forall y \in \mbox{Vars}. \ddep{y}(\trlet (x,
%   \tr_1, \tr_2)  ) \leq
% \dmap'(y)$ proved by $(3)$ and $(9)$. \\
% 3. $(\stepiA - j_1 -j_2, \valr_2 )  \in \lrv{ 
%     \type }$, proved by $(10)$.\\

% \end{proof}

%%%%%%%%%%%%%%%%%%%%%%%%%%%%%%%%%%%%%%%%%%%%%%%%%%%%%%%%%%%%%%%%%%%%%%%%%%%%%%%%%%%%%%%%%%%%%%%%%%%%%%%%%%
%END the Proof of old Fundamental Theorem 
%%%%%%%%%%%%%%%%%%%%%%%%%%%%%%%%%%%%%%%%%%%%%%%%%%%%%%%%%%%%%%%%%%%%%%%%%%%%%%%%%%%%%%%%%%%%%%%%%%%%%%%%%%
