\clearpage
\begin{lem} \label{lem:adap_depth_zero}
 if $\adap(\tr) = 0 $ then for all variable x, $\ddep{x}(\tr) \leq 0
 $. ($\bot$ is less than any number in $\mathbb{N}$).
\end{lem}
\begin{proof}
\wq{ It is proved simply by induction on $(\tr)$.}
\end{proof}

\begin{lem} \label{lem:delta_free}
  if $\env, \expr
    \bigstep \valr,  \tr $ and $\delta \not \in \expr$ and $\delta \not
    \in \env$, then $ \adap(\tr)   = 0 $ and $\delta \not \in \valr $
\end{lem}
\begin{proof}
\wq{By induction on the derivation of opertational semantics.\\}
%
\textbf{Case} 
\[\inferrule{ }{\env, x \bigstep \env(x), (x, \env ) }\]
We know $\delta \not\in \env \conj \delta \not\in x$, \\
so we know : 
$ \tr = (x, \env) \Rightarrow  \adap(\tr) = 0$ and $\delta \not \in
\env(x) $. \\
%
\textbf{Case}
\[
\inferrule{
    \env, \expr_1 \bigstep \valr_1, \tr_1 \\
    \valr_1 = (\efix f(x).\expr, \env') \\\\
    \env, \expr_2 \bigstep \valr_2, \tr_2 \\
    \env'[f \mapsto \valr_1, x \mapsto \valr_2], \expr \bigstep \valr, \tr
  }{
    \env, \expr_1 \eapp \expr_2 \bigstep \valr, \trapp{\tr_1}{\tr_2}{f}{x}{\tr}
  }
\]
We know that: $ \delta \not\in (\expr_1 \eapp \expr_2) ~(1)\conj \delta
\not\in \env $. \\
From $(1)$, we get : $\delta \not\in \expr_1~(2)$ and $\delta \not\in
\expr_2~(3)$.\\
IH on the first premise instantiated with $(2)$, we know:
$\adap(\tr_1) = 0 \conj \delta \not\in \valr_1~(4)$. \\
Because $\valr_1$ is a function, we know that $\delta \not\in (\efix
f(x).\expr, \env') ~(5)$ from the second premise. \\
IH on the third premise instantiated with $(3)$, we know:
$\adap(\tr_2) = 0 \conj \delta \not\in \valr_2~(6)$. \\

From $(4), (5), (6)$, we know that:
 $ \delta \not\in \env'[f \mapsto \valr_1, x \mapsto \valr_2]$ and $
 \delta \not\in \expr~(7) $. \\

By IH on the fourth premise instantiated with $(7)$, we conclude that
:
$\delta \not\in \valr $ and $\adap(\tr) = 0$. \\

We want to show: \\
 $ \adap(\trapp{\tr_1}{\tr_2}{f}{x}{\tr_3})  = 
      \adap(\tr_1) + \max (\adap(\tr_3), \adap(\tr_2) +
      \ddep{x}(\tr_3)) = 0$. \\
We already know that $ \adap(\tr_1) =0 \conj\adap(\tr_2) =0  \conj
\adap(\tr_1) =0 $. \\
By Lemma~\ref{lem:adap_depth_zero}, we know: $\ddep{x}(\tr_3) \leq 0$.\\
So we conclude that $\adap(\trapp{\tr_1}{\tr_2}{f}{x}{\tr_3}) =0$.\\
%
\textbf{Case}
\[\inferrule{
  }{
    \env, \efix f(x). \expr \bigstep (\efix f(x).\expr, \env),
    (\trfix f(x).\expr, \env)
  }\]
We assume that $\delta \not\in \env$ and $\delta \not\in \efix
f(x). \expr$.\\
STS1: $\adap(\tr) = \adap( (\trfix f(x).\expr, \env) ) = 0$, which is
proved by the defintion of adaptivity. \\
STS2: $\delta \not\in (\efix f(x).\expr, \env)$,  which is known by
our assumption. \\
%
\textbf{Case}
\[
\inferrule{
    \env, \expr_1 \bigstep \valr_1, \tr_1 \\
    \env, \expr_2 \bigstep \valr_2, \tr_2
  }{
    \env, (\expr_1, \expr_2) \bigstep (\valr_1, \valr_2), (\tr_1, \tr_2)
  }
\]
We assume that $\delta \not\in \env$ and $\delta \not\in  (\expr_1, \expr_2)~(1) $.\\
From $(1)$, we can infer that : $\delta \not\in \expr_1~(2)$ and $\delta
\not\in \expr_2~(3)$.\\
By IH on the first premise instantiated with $(2)$, we know:
$\adap(\tr_1) = 0~(4)$ and $\delta \not\in \valr_1~(5) $. \\
By IH on the first premise instantiated with $(3)$, we know:
$\adap(\tr_2) = 0~(6)$ and $\delta \not\in \valr_2~(7)$. \\
STS1: $\adap((\tr_1,\tr_2)) = 0$, which is proved by $(4),(6)$.\\
STS2: $\delta \not\in (\valr_1,\valr_2) $, which is proved by
$(5),(7)$.\\

%
\textbf{Case}
\[
\inferrule{
    \env, \expr \bigstep (\valr_1, \valr_2), \tr
  }{
    \env, \eprojl(\expr) \bigstep \valr_1, \trprojl(\tr)
  }
\]
We assume that $\delta \not\in \env$ and $\delta \not\in
\eprojl(\expr) ~(1) $.\\
From $(1)$, we can infer that : $\delta \not\in \expr~(2)$ \\
 By IH on the first premise instantiated with $(2)$, we know:
$\adap(\tr) = 0~(3)$ and $\delta \not\in (\valr_1, \valr_2) ~(4) $. \\
STS1: $\adap(\trprojl(\tr) ) = 0$, which is proved by $(3)$.\\
STS2: $\delta \not\in \valr_1 $, which is proved by $(4)$. \\

%
\textbf{Case}
\[
\inferrule{
  \env, \expr_1 \bigstep \valr_1, \tr_1 \\
  \env[x \mapsto \valr_1] , \expr_2 \bigstep \valr, \tr_2
}
{\env, \elet x;q = \expr_1 \ein \expr_2 \bigstep \valr, \trlet (x,
  \tr_1, \tr_2) }
\]
We assume that $\delta \not\in \env$ and $\delta \not\in
\elet x;q = \expr_1 \ein \expr_2 ~(1) $.\\
From $(1)$, we can infer that : $\delta \not\in \expr_1~(2)$ and $\delta \not\in \expr_2~(3)$.  \\
By IH on the first premise instantiated with $(2)$, we know:
$\adap(\tr_1) = 0~(4)$ and $\delta \not\in \valr_1 ~(5) $. \\
From $(5)$, We know that $ \delta \not\in \env[x \mapsto
\valr_1]~(6)$.\\
By IH on the second premise instantiated with $(3),(6)$ , we know:
$\adap(\tr_2) = 0~(7)$ and $\delta \not\in \valr~(8)$. \\
STS1: $\adap( \trlet (x,
  \tr_1, \tr_2) ) = 0$, which is proved by $(4),(7)$ and Lemma~\ref{lem:adap_depth_zero}.\\
STS2: $\delta \not\in \valr_1 $, which is proved by $(8)$. \\

\end{proof}

\begin{lem}\label{lem:sub_sound} \wq{\textsf{Sutyping Soundness}} \\
1. If $ \Delta \models \sub{ \type }{ \type' } $ and $ \ienv \in \lrv{\Delta}$ and  $(\stepiA, \valr) \in \lrv{\ienv \type}$,  then  $(\stepiA, \valr) \in \lrv{\ienv \type'}$.
  \\
 2. If $ \Delta \models \sub{ \type }{ \type' } $ and $ \ienv \in
 \lrv{\Delta}$ and  $(\stepiA, (\env, \expr)) \in
 \lre{\dmap}{\nnatA}{\ienv \type}$, and $\dmap < \dmap'$ and $\nnatA < \nnatA' $,  then  $(\stepiA, (\env, \expr)) \in \lre{\dmap'}{\nnatA'}{\ienv \type'}$.
   \\
\end{lem}
%
\begin{proof} The proof of statement (1) is by induction on the
  subtying derivation.\\

\textbf{Case}
\[ 
 \inferrule{
     \Delta \models \sub{\type_1 }{ \type_1'  } \\
         \Delta \models \sub{\type_2 }{ \type_2'  }
    }{
       \Delta \models \sub{\type_1 \times \type_2 }{ \type_1' \times \type_2'  }
    }
\]
Suppose we know : $ (\stepiA, (\valr_1, \valr_2)) \in \lrv{\ienv \type_1 \times \type_2} $.\\
TS:  $ (\stepiA, (\valr_1, \valr_2)) \in \lrv{\ienv \type_1' \times \type_2'} $ \\
Unfold its definition, we know: $  (\stepiA, \valr_1 ) \in \lrv{\ienv \type_1} $ and $  (\stepiA, \valr_2 ) \in \lrv{\ienv \type_2} $.\\
By IH on the first premise, we know: $  (\stepiA, \valr_1 ) \in \lrv{\ienv \type_1'} $.\\
By IH on the second premise, we know: $  (\stepiA, \valr_2 ) \in \lrv{\ienv \type_2'} $.\\
This case is proved.\\

\textbf{Case}
\[
     \inferrule
    {
      \Delta  \models \sub{ \type_1' }{ \type_1 }
      \and
      \Delta  \models \sub{ \type_2 }{ \type_2' }
      \and
      \dmap \leq \dmap'
      \and
      \nnatA \leq \nnatA'
      \and 
      q \leq q'
    }
    {
      \Delta  \models \sub{ \tarr{\type_1}{\type_2}{ \nnatbiA }{\dmap}{\nnatA} }
      { \tarr{\type_1'}{\type_2'}{\nnatbiA'}{\dmap'}{\nnatA'} }
    }
\]
Suppose  $ (\stepiA, (\efix f(x).\expr, \env) ) \in \lrv{\ienv (\tarr{\type_1}{\type_2}{\nnatbiA}{\dmap}{\nnatA})  } ~(\star)$.\\
TS: $ (\stepiA, (\efix f(x).\expr, \env) ) \in \lrv{\ienv (\tarr{\type_1'}{\type_2'}{\nnatbiA'}{\dmap'}{\nnatA'})  } $ \\
From $(\star)$, we know:\\
$\forall \stepiB < \stepiA.\eapp  \forall (\stepiB, \valr) \in \lrv{\type_1}. $ \\
$ (\stepiB, (\env[x \mapsto \valr, f \mapsto (\efix f(x).\expr, \env)], \expr)) \in \lre{\dmap[x: \nnatbiA, f: \infty]}{\nnatA}{\type_2} $\\
STS:
$\forall \stepiB < \stepiA.\eapp  \forall (\stepiB, \valr') \in \lrv{\type_1'}. $ \\
$ (\stepiB, (\env[x \mapsto \valr', f \mapsto (\efix f(x).\expr, \env)], \expr)) \in \lre{\dmap'[x: \nnatbiA, f: \infty]}{\nnatA'}{\type_2'} ~(\diamond)$\\
Pick j, assume $(\stepiB, \valr') \in \lrv{\tau_1'}$, we also know $(\stepiB, \valr') \in \lrv{\tau_1}$ by IH on the first premise.\\
From $(\star)$, we know: \\
$ (\stepiB, (\env[x \mapsto \valr', f \mapsto (\efix f(x).\expr, \env)], \expr)) \in \lre{\dmap[x: \nnatbiA, f: \infty]}{\nnatA}{\type_2} $.\\
Unfold its definition, we get: \\
$ \forall \valr_t \eapp  \tr\eapp  \stepiB.\eapp \env[x \mapsto \valr', f \mapsto (\efix f(x).\expr, \env)], \expr \bigstep \valr_t, \tr  \conj (\size{\tr} = \stepiB) \conj (\stepiB \leq \stepiA)$\\
$\Rightarrow (\adap(\tr) \leq \nnatA \conj \forall x \in \mbox{Vars}.\eapp  \ddep{x}(\tr) \leq \dmap[x:\nnatbiA, f: \infty](x) \conj ((\stepiA - \stepiB,  \valr_t) \in \lrv{\type_2})$\\
Unfold $(\diamond)$, STS:
\begin{enumerate}
\item  $\adap(\tr) \leq \nnatA'$, It is proved because we know $\adap(\tr) \leq \nnatA $ and $\nnatA \leq \nnatA'$. \\
\item $\forall x \in \mbox{Vars}.\eapp  \ddep{x}(\tr) \leq \dmap'[x:\nnatbiA', f: \infty](x) $, because $\dmap \leq \dmap'$, It is proved using $\forall x \in \mbox{Vars}.\eapp  \ddep{x}(\tr) \leq \dmap[x:\nnatbiA, f: \infty](x) $ . \\
\item $((\stepiA - \stepiB,  \valr_t) \in \lrv{\type_2'})$ it is proved by IH on the second premise with $ ((\stepiA - \stepiB,  \valr_t) \in \lrv{\type_2})$. \\
\end{enumerate}




% \textbf{case}
% \[
%  \inferrule{
% \dmap' \leq \dmap
%     }{
%        \Delta \models \sub{\tarr{\type_1}{\type_2}{0}{\dmap'}{0} }{  \tbox{(
%           \tarr{\type_1}{\type_2}{\nnatbiA}{\dmap}{\nnatA} )  }
%     } }
% \]
% Suppose  $ (\stepiA, (\efix f(x).\expr, \env) ) \in \lrv{\ienv (\tarr{\type_1}{\type_2}{0}{\dmap'}{0})  } ~(\star)$.\\
% TS: $ (\stepiA, (\efix f(x).\expr, \env) ) \in \lrv{ \tbox{\ienv (\tarr{\type_1}{\type_2}{\nnatbiA}{\dmap}{\nnatA})  } } $ \\
% Unfold its defintion, STS:\\
% 1. $ \delta \not \in  (\efix f(x).\expr, \env)$ . \wq{I do not know how to prove it.} \\
% 2.  $(\stepiA, (\efix f(x).\expr, \env) ) \in  \lrv{(\tarr{\type_1}{\type_2}{\nnatbiA}{\dmap}{\nnatA})}
% $.  It can be proved from $(\star)$ because $ \Delta \models \sub{
%   (\tarr{\type_1}{\type_2}{0}{\dmap'}{0})} {
%   (\tarr{\type_1}{\type_2}{\nnatbiA}{\dmap}{\nnatA}) }  $ \\

% \textbf{case}
% \[
%  \inferrule{
% \dmap' \leq \dmap
%     }{
%        \Delta \models \sub{\tarr{\tbox{\type_1}}{\tbox{\type_2}}{0}{\dmap'}{0} }{  \tbox{(
%           \tarr{\type_1}{\type_2}{\nnatbiA}{\dmap}{\nnatA} )  }
%     } }
% \]
% Suppose  $ (\stepiA, (\efix f(x).\expr, \env) ) \in \lrv{\ienv
%   (\tarr{\tbox{\type_1}}{\tbox{\type_2}}{0}{\dmap'}{0})  }
% ~(\star)$.\\
% Unfold $(\star)$, we pick $\stepiB < \stepiA$ and $(\stepiB, \valr)
% \in \lrv{\tbox{\type_1}}$. \\
% We get:
%  \[
%    (\stepiB, (\env[x \mapsto \valr, f \mapsto (\efix f(x).\expr, \env)], \expr)) \in \lre{\dmap'[x: 0, f: \infty]}{0}{\tbox{\type_2}}
% \]
% Unrolling its defintion,\\
% $ \forall \valr_t \eapp  \tr\eapp  \stepiB.\eapp \env[x \mapsto \valr, f \mapsto (\efix f(x).\expr, \env)], \expr \bigstep \valr_t, \tr  \conj (\size{\tr} = \stepiB) \conj (\stepiB \leq \stepiA)$\\
% $\Rightarrow (\adap(\tr) \leq 0 \conj \forall x \in \mbox{Vars}.\eapp
% \ddep{x}(\tr) \leq \dmap[x:0, f: \infty](x) \conj ((\stepiA - \stepiB,
% \valr_t) \in \lrv{\tbox{ \type_2} })~(\diamond)$\\

% TS: $ (\stepiA, (\efix f(x).\expr, \env) ) \in \lrv{ \tbox{\ienv
%     (\tarr{\type_1'}{\type_2'}{\nnatbiA}{\dmap}{\nnatA})  } } $ \\
% Unfold its defintion, STS:\\
% 1. $ \delta \not \in  (\efix f(x).\expr, \env)$ . \wq{I do not know how to prove it.} \\
% 2.  $(\stepiA, (\efix f(x).\expr, \env) ) \in  \lrv{(\tarr{\type_1}{\type_2}{\nnatbiA}{\dmap}{\nnatA})}
% $. \\
%    Use $\stepiB$ and $\valr$.\\
%     STS:  \[
%    (\stepiB, (\env[x \mapsto \valr, f \mapsto (\efix f(x).\expr, \env)], \expr)) \in \lre{\dmap[x: \nnatbiA, f: \infty]}{\nnatA}{\type_2}
% \]
% It is proved by $(\diamond)$.
%  \\



\textbf{Case}
\[
\inferrule{
       % \forall x \in \dmap'. \dmap'(x) =0
    }{
       \Delta \models \sub{\tbox{(
          \tarr{\type_1}{\type_2}{\nnatbiA}{\dmap'}{\nnatA} )} 
      }{\tarr{(\tbox{\type_1}) }{(\tbox{\type_2})}{0}{\dmap'}{0} }
    }
\]
Assume $ \ienv \in \lrv{\Delta}$.\\
We have:  $$ (\stepiA, (\efix f(x).\expr, \env) ) \in \lrv{\ienv \tbox{(
          \tarr{\type_1}{\type_2}{\nnatbiA}{\dmap'}{\nnatA} )} }
      ~(\star)$$
TS: $ (\stepiA, (\efix f(x).\expr, \env) ) \in \lrv{ \ienv 
  \tarr{(\tbox{\type_1}) }{(\tbox{\type_2})}{0}{\dmap'}{0}} $ \\
Assume $\stepiB < \stepiA \conj (j, \valr) \in \lrv{\tbox{\type_1}}$,
which implies $ (j, \valr) \in \lrv{\type_1} \conj \delta \not \in \valr$ \\
STS: $(\stepiB, (\env[x \mapsto \valr, f \mapsto (\efix f(x).\expr,
\env)], \expr)) \in \lre{\dmap[x: 0, f:
  \infty]}{0}{ \tbox{ \type_2} } (\star\star)$\\

By unrolling $(\star)$, we know that: 
 $$ (\stepiA, (\efix f(x).\expr, \env) ) \in \lrv{\ienv (
          \tarr{\type_1}{\type_2}{\nnatbiA}{\dmap'}{\nnatA} ) } ~(a) \conj
        \delta \not \in   (\efix f(x).\expr, \env) ~(b)
      $$

By unrolling $(a)$ with $\stepiA < \stepiB \conj (j, \valr) \in
\lrv{\type_1}$, we get:
 \[
(\stepiB, (\env[x \mapsto \valr, f \mapsto (\efix f(x).\expr,
\env)], \expr)) \in \lre{\dmap'[x: \nnatbiA, f:
  \infty]}{\nnatA}{  \type_2 } (\diamond)
\]

Unrolling $(\diamond)$, assume \[ \env[x \mapsto \valr, f \mapsto (\efix f(x).\expr,
\env)], \expr \bigstep \valr_1, \tr_1 \conj |\tr_1| = \stepiB_1 \conj
\stepiB_1 \leq \stepiA \] .
We get : $$ \adap(\tr_1) \leq \nnatA ~(c)$$
         $$\forall y \in \mbox{Vars}.\eapp  \ddep{y}(\tr_1) \leq
         \dmap'[x: \nnatbiA, f: \infty](x) ~(d)$$
         $$  (\stepiA - \stepiB_1,  \valr_1) \in \lrv{\type_2}~(e) $$

Unrolling $(\star\star)$ with our assumption $ \env[x \mapsto \valr, f \mapsto (\efix f(x).\expr,
\env)], \expr \bigstep \valr_1, \tr_1 \conj |\tr_1| = \stepiB_1 \conj
\stepiB_1 \leq \stepiA $. \\ 
We know that $\delta \not\in \valr \conj \delta \not\in  (\efix f(x).\expr,
\env) \conj \delta \not\in \expr $, by Lemma~\ref{lem:delta_free}, we
conclude that: $\adap(\tr_1) =0~(1)$ and  $ \delta \not \in \valr_1~(2)$.
 STS:
\begin{enumerate}
\item $ \adap(\tr_1) \leq 0 $, proved by $(1)$ \\  

\item $\forall y \in \mbox{Vars}.\eapp  \ddep{y}(\tr_1) \leq
         \dmap'[x: 0, f: \infty](x)$ . By
         Lemma~\ref{lem:adap_depth_zero} and $(1)$, we can show that
         $\ddep{x}(\tr_1) = 0 
leq \dmap'[x: 0, f: \infty](x) $ when $y = x$.\\
           When $y \not= x$, it is proved by $(d)$    \\

\item $  (\stepiA - \stepiB_1,  \valr_1) \in \lrv{\tbox {\type_2} }$
  \\
It is proved by $(e)$ and $(2)$.
\end{enumerate}

\textbf{Case}
 \[
 \inferrule*[right=list]{
      \Delta \models \sub{ \tau_1  }{ \tau_2 } 
    }{
      \Delta \models \sub{ \tlist{\tau_1}  }{ \tlist{\tau_2} }
    }
\]
Assume $ \ienv \in \lrv{\Delta}$.\\
There are two subcases. \\
\begin{enumerate}
\item  $ (\stepiA, \enil ) \in \lrv{\ienv(  \tlist{\tau_1} ) }$ \\
       It is proved that $ (\stepiA, \enil ) \in \lrv{\ienv(
         \tlist{\tau_2})  }$ by the definition.\\
\item   $  (\stepiA, \econs(\valr_1,\valr_2) ) \in \lrv{\ienv (
    \tlist{\tau_1}) } $ \\
      We know that $ (\stepiA, \valr_1) \in \lrv{\ienv (\type_1)}~(\star) $ and
      $(\stepiA, \valr_2) \in \lrv{\ienv (\tlist{\type_1} ) }~(\diamond)$.\\
     By IH on $(\star)$, we know that $(\stepiA, \valr_1) \in
     \lrv{\ienv \type_2} $.\\
    STS: $(\stepiA, \valr_2) \in \lrv{\ienv ( \tlist{\type_2} ) }$, which is
    proved by IH on $(\diamond)$.
\end{enumerate}

\textbf{Case}
 \[
 \inferrule*[right=listbox]
    {
      \empty
    }
    {
      \Delta \models \sub{ \tlist{\tbox{\tau }}  }{ \tbox{\tlist{\tau}} } 
    }
\]
Assume $ \ienv \in \lrv{\Delta}$.\\
There are two subcases. \\
\begin{enumerate}
\item  $ (\stepiA, \enil ) \in \lrv{\ienv ( \tlist{\tbox{\tau} })  }$ \\
       It is proved that $ (\stepiA, \enil ) \in \lrv{\ienv ( \tbox{
         \tlist{\tau} } )  }$ because $ \delta \not\in \enil$ and $(\stepiA, \enil ) \in \lrv{\ienv  \tlist{\tau }  }  $.\\
\item   $  (\stepiA, \econs(\valr_1,\valr_2) ) \in \lrv{\ienv (
    \tlist{  \tbox {\tau_1} } ) } $ \\
      We know that $ (\stepiA, \valr_1) \in \lrv{ \tbox{ \ienv \type
        } } 
~(\star) $ and
      $(\stepiA, \valr_2) \in \lrv{  \tlist{  \tbox{  \ienv \type}
        } }  ~(\diamond)$.\\
      Unfold $(\star)$, we know : $ \delta \not\in \valr_1~(a)$ and $ (\stepiA, \valr_1) \in \lrv{ \ienv \type
         }~(b)  $. \\
      By IH on $(\diamond)$, we know that :  $(\stepiA, \valr_2) \in
      \lrv{ \tbox{ \tlist{   \ienv \type  } } }  $.\\
      Unfolt its defintion, we know that $\delta \not\in \valr_2~(c)$
      and $(\stepiA, \valr_2) \in
      \lrv{  \tlist{   \ienv \type  }  }~(d)$ . \\
     STS1: $  (\stepiA, \econs(\valr_1,\valr_2) ) \in \lrv{\ienv (
    \tlist{  \tau } ) } $.\\
           It is proved by (b),(d).\\
     
     STS2: $ \delta \not\in
  \econs(\valr_1,\valr_2) $. \\
    It is proved by (a), (c).\\
     By IH on $(\star)$, we know that $(\stepiA, \valr_1) \in
     \lrv{\type_2} $.\\
    STS: $(\stepiA, \valr_2) \in \lrv{\tlist{\type_2}}$, which is
    proved by IH on $(\diamond)$.
\end{enumerate}

  

\textbf{The proof of statement (2)} \\
Assume $(\stepiA, (\env, \expr)) \in
 \lre{\dmap}{\nnatA}{\ienv \type}~(\star)$. \\
%


TS: $(\stepiA, (\env, \expr)) \in
 \lre{\dmap'}{\nnatA'}{\ienv \type'}$.\\
Unfold its definition, STS:
$ \forall \stepiB, \env, \tr.  \env, \expr \bigstep \valr, \tr \conj
(\size{\tr} = \stepiB) \conj (\stepiB \leq \stepiA) $.\\
$\Rightarrow \adap(\tr) \leq \nnatA' \conj$\\
$\forall x \in \mbox{Vars}.\eapp  \ddep{x}(\tr) \leq \dmap'(x)\conj$\\
$ (\stepiA - \stepiB,  \valr) \in \lrv{\type'}$\\
%
Pick  $\stepiB$,$\valr$,  $\tr$, s.t.
$\env, \expr \bigstep \valr, \tr \conj
(\size{\tr} = \stepiB) \conj (\stepiB \leq \stepiA) $.\\
STS1: $\adap(\tr) \leq \nnatA' $ \\
STS2: $\forall x \in \mbox{Vars}.\eapp  \ddep{x}(\tr) \leq
\dmap'(x)$\\
STS3: $ (\stepiA - \stepiB,  \valr) \in \lrv{\type'}  $.\\


By inversion on the assumption $(\star)$, Pick $\stepiB$,$\valr$,
$\tr$. we know from assumption: $ \env, \expr \bigstep \valr, \tr \conj
(\size{\tr} = \stepiB) \conj (\stepiB \leq \stepiA) $.\\
We get: $\adap(\tr) \leq \nnatA ~(a)$\\
$\forall x \in \mbox{Vars}.\eapp  \ddep{x}(\tr) \leq \dmap(x)~(b)$\\
$ (\stepiA - \stepiB,  \valr) \in \lrv{\type}~(c)$\\

STS1: $\adap(\tr) \leq \nnatA' $ is proved by $(a)$ and $\nnatA \leq
\nnatA'$. \\
STS2: $\forall x \in \mbox{Vars}.\eapp  \ddep{x}(\tr) \leq
\dmap'(x)$. It is proved by $(b)$ and $\dmap \leq \dmap'$. \\
STS3: $ (\stepiA - \stepiB,  \valr) \in \lrv{\type'}$. It is proved by
IH1 instantiated with $(c)$  and $ \Delta \models \sub{\type}{\type'}$.\\


\end{proof}