\section{Examples for \cite{cousot2019abstract}}
\begin{example}
\[
 \begin{array}{l}
 \mathcal{S}^{*}\sem{
 \ewhile {}^0 (x > 0) {}^1 x = x - 1;
 } \triangleq \mathsf{lfp}^\subseteq\mathcal{F}^*\sem{\ewhile {}^0 (x > 0) {}^1 x = x - 1;}
  \end{array}
 \]
 Let $X_0 =  \emptyset$
 \[
 \begin{array}{l}
X_1 = 
\mathcal{F}^*\sem{\ewhile {}^0 (x > 0) {}^1 x = x - 1;}(X_0) = \left\{ \left< \pi_1^0, ^0\right> \mid \pi_1^0 \in \mathbb{T^{+}} \right\}
  \end{array}
 \]
 % Let $X_1 =  \left\{ \left< \pi_1^0, ^0\right> \mid \pi_1^0 \in \mathbb{T^{+}} \right\}$
 \[
 X_2 = \begin{array}{l}
 \mathcal{F}^*\sem{\ewhile {}^0 (x > 0) {}^1 x = x - 1;}(X_1) = X_1
  \\
 \quad \cup \left\{ \left< \pi_1^0, {}^0 \xrightarrow{\neg(x > 0)} {}^{\mathsf{aft}\sem{S}} \right> 
 \mid \pi_1^0 \in \mathbb{T^{+}} \land 
 \sem{(x > 0)}\env(\pi_1^0) = \efalse \right\}
\\
 \quad \cup \left\{ \left< \pi_1^0, {}^0 \xrightarrow{(x > 0)} {}^1 \right> 
 \mid \pi_1^0 \in \mathbb{T^{+}} \land 
 \sem{(x > 0)}\env(\pi_1^0) = \etrue \right\}
 \\
 \quad \cup \left\{ \left< \pi_1^0, {}^0 \xrightarrow{(x > 0)} {}^1 \xrightarrow{(x = x - 1) = v} {}^0 \right> 
 \mid \pi_1^0 \in \mathbb{T^{+}} \land 
 \sem{(x > 0)}\env(\pi_1^0) = \etrue  \land
 \sem{(x - 1)}\env(\pi_1^0 \xrightarrow{(x > 0)} {}^1) = v \right\}
 \end{array}
 \]
  \[
 X_3 = \begin{array}{l}
 \mathcal{F}^*\sem{\ewhile {}^0 (x > 0) {}^1 x = x - 1;}(X_2) = X_2
  \\
  \quad \cup \Big\{ \left< \pi_1^0, {}^0 \xrightarrow{(x > 0)} {}^1 \xrightarrow{x = v} {}^0 \xrightarrow{(x > 0)} {}^1 \right> 
 \mid \pi_1^0 \in \mathbb{T^{+}} \land 
 \sem{(x > 0)}\env(\pi_1^0) = \etrue  
 \\ \qquad \land
 \sem{(x - 1)}\env(\pi_1^0 \xrightarrow{(x > 0)} {}^1) = v
 \land 
 \sem{(x > 0)}\env(\pi_1{}^0 \xrightarrow{(x > 0)} {}^1 \xrightarrow{x = v} {}^0) = \etrue  \Big\}
  \\
	\quad \cup \Big\{ \left< \pi_1^0, {}^0 \xrightarrow{(x > 0)} {}^1 \xrightarrow{x = v} {}^0 \xrightarrow{(x > 0)} {}^1 \xrightarrow{x = v'} {}^0 \right> 
 \mid \pi_1^0 \in \mathbb{T^{+}} \land 
 \sem{(x > 0)}\env(\pi_1^0) = \etrue  \land
 \sem{(x - 1)}\env(\pi_1^0 \xrightarrow{(x > 0)} {}^1) = v
 \\ \qquad \land 
 \sem{(x > 0)}\env(\pi_1{}^0 \xrightarrow{(x > 0)} {}^1 \xrightarrow{x = v} {}^0) = \etrue  \land
 \sem{(x - 1)}\env(\pi_1^0 \xrightarrow{(x > 0)} {}^1 \xrightarrow{x = v} {}^0 \xrightarrow{(x > 0)} {}^1) = v' \Big\}
  \\
 	\quad \cup \Big\{ \config{\pi_1^0, 
  {}^0 \xrightarrow{(x > 0)} {}^1 \xrightarrow{x = v} {}^0 
  \xrightarrow{\neg(x > 0)} {}^{\mathsf{aft}\sem{S}}}
 \mid \pi_1^0 \in \mathbb{T^{+}} \land 
 \sem{(x > 0)}\env(\pi_1^0) = \etrue  \land
 \sem{(x - 1)}\env(\pi_1^0 \xrightarrow{(x > 0)} {}^1) = v 
 \\ \qquad \land 
 \sem{(x > 0)}\env(\pi_1{}^0 \xrightarrow{(x > 0)} {}^1 \xrightarrow{x = v} {}^0) = \efalse
 \Big\}
\\
 \end{array}
 \]
 %
 Let $X_p$ be the set such that:
 \[
 \mathcal{F}^*\sem{\ewhile {}^0 (x > 0) {}^1 x = x - 1;}(X_p) = X_p
 \]
 %
 Then, $X_p$ is the least fixed point as follows, and 
 $X_p = \mathcal{S}^{*}\sem{\ewhile {}^0 (x > 0) {}^1 x = x - 1;}$
 %
 \[
 \begin{array}{l}
 X_p = \left\{ \left< \pi_1^0, ^0\right> \mid \pi_1^0 \in \mathbb{T^{+}} \right\}
 \\
  \quad \cup \left\{ \left< \pi_1^0, {}^0 \xrightarrow{(x > 0)} {}^1 \right> 
 \mid \pi_1^0 \in \mathbb{T^{+}} \land 
 \sem{(x > 0)}\env(\pi_1^0) = \etrue \right\}
 \\  \quad \cup 
  \left\{ \left< \pi_1^0, {}^0 \xrightarrow{(x > 0)} {}^1 \xrightarrow{(x = x - 1) = v} {}^0 \right>
 \mid \pi_i^0 \in \mathbb{T^{+}} \land 
 \sem{(x > 0)}\env(\pi_1^0) = \etrue  \land
 \sem{(x - 1)}\env(\pi_1^0 \xrightarrow{(x > 0)} {}^1) = v \right\}
 \\ \quad \cup 
 \Big\{ \left< \pi_1^0, {}^0 \xrightarrow{(x > 0)} {}^1 \xrightarrow{x = v} {}^0 \xrightarrow{(x > 0)} {}^1 \right> 
 \mid \pi_1^0 \in \mathbb{T^{+}} \land 
 \sem{(x > 0)}\env(\pi_1^0) = \etrue  
 \\ \qquad \land
 \sem{(x - 1)}\env(\pi_1^0 \xrightarrow{(x > 0)} {}^1) = v
 \land 
 \sem{(x > 0)}\env(\pi_1{}^0 \xrightarrow{(x > 0)} {}^1 \xrightarrow{x = v} {}^0) = \etrue  \Big\}
  \\ \quad \cup  
  \left\{ \left< \pi_1^0, {}^0 \xrightarrow{(x > 0)} {}^1 \xrightarrow{(x = x - 1) = v_1} {}^0 \xrightarrow{(x > 0)} {}^1 \xrightarrow{(x = x - 1) = v_2} {}^0 \right> 
 \left \vert 
 \begin{array}{l}
 \pi_i^0 \in \mathbb{T^{+}} \\
 \land 
 \sem{(x > 0)}\env(\pi_1^0) = \etrue  \\
 \land
 \sem{(x - 1)}\env(\pi_1^0 \xrightarrow{(x > 0)} {}^1) = v_1 \\
 \land 
 \sem{(x > 0)}\env(\pi_1{}^0 \xrightarrow{(x > 0)} {}^1 \xrightarrow{(x = x - 1) = v_1} {}^0) = \etrue \\
 \land
 \sem{(x - 1)}\env(\pi_1^0 \xrightarrow{(x > 0)} {}^1 \xrightarrow{(x = x - 1) = v_1} {}^0 \xrightarrow{(x > 0)} {}^1) = v_2
 \end{array}
 \right.
 \right\}
 \\ \quad  \cup  \cdots 
 \\ \quad \cup  
 \left\{ \left< \pi_1^0, {}^0 \xrightarrow{\neg(x > 0)} {}^{\mathsf{aft}\sem{S}} \right> 
 \mid \pi_1^0 \in \mathbb{T^{+}} \land 
 \sem{(x > 0)}\env(\pi_1^0) = \efalse \right\}
 \\  \quad \cup 
  \Big\{ \config{\pi_1^0, 
  {}^0 \xrightarrow{(x > 0)} {}^1 \xrightarrow{x = v} {}^0 
  \xrightarrow{\neg(x > 0)} {}^{\mathsf{aft}\sem{S}}}
 \mid \pi_1^0 \in \mathbb{T^{+}} \land 
 \sem{(x > 0)}\env(\pi_1^0) = \etrue  \land
 \sem{(x - 1)}\env(\pi_1^0 \xrightarrow{(x > 0)} {}^1) = v 
 \\ \qquad \land 
 \sem{(x > 0)}\env(\pi_1{}^0 \xrightarrow{(x > 0)} {}^1 \xrightarrow{x = v} {}^0) = \efalse
 \Big\}
 \\ \quad \cup  \cdots 
 \\\quad \cup  \left\{ \left< \pi_1^0, {}^0 \xrightarrow{(x > 0)} {}^1\xrightarrow{(x = x - 1) = v_1} {}^0 \cdots  {}^0 \xrightarrow{\neg(x > 0)} {}^{\mathsf{aft}\sem{S}} \right>  
 \left \vert 
 \begin{array}{l}
 \pi_1^0 \in \mathbb{T^{+}}\\
 \land 
 \sem{(x > 0)}\env(\pi_1^0) = \etrue  \\
 \land
 \sem{(x - 1)}\env(\pi_1^0 \xrightarrow{(x > 0)} {}^1) = v_1 \\
 \land \cdots \\
 % \land
 % \sem{(x - 1)}\env(\pi_1^0 \xrightarrow{(x > 0)} {}^1 \xrightarrow{(x = x - 1) = v} {}^0 \xrightarrow{(x > 0)} {}^1) = v_2\\
 \land 
 \sem{(x > 0)}\env(\pi_i{}^0 \xrightarrow{(x > 0)} {}^1\xrightarrow{(x = x - 1) = v_1} {}^0 \cdots  {}^0) = \efalse
 \end{array}
 \right.
 \right\}
 \end{array}
 \]
 %
 Using a symbolic representation for $X_p$, we have:
 \[
 \begin{array}{ll}
 X_p &=  \left\{ \left< \pi_1^0, ^0\right> \mid \pi_1^0 \in \mathbb{T^{+}} \right\}
 \\ &  \cup 
 \left\{ \left< \pi_1^0, {}^0 \pi_{s_1} {}^0 \cdots {}^0 \pi_{s_v} {}^0\right>
 \mid \pi_i^0 \in \mathbb{T^{+}} \land v \in \mathbb{N} \land
 \sem{x}\env(\pi_1^0) = v
 \land v > 0  \land
 {}^0 \pi_{s_i} {}^0 = {}^0 \xrightarrow{(x > 0)} {}^1 \xrightarrow{x = v - i} {}^0\right\}
 \\ &  \cup 
 \left\{ \left< \pi_1^0, {}^0 \pi_{s_0} {}^0 \cdots {}^0 \pi_{s_{v - 1}} {}^0 \xrightarrow{(x > 0)} {}^1 \right>
 \mid \pi_i^0 \in \mathbb{T^{+}} \land v \in \mathbb{N} \land
 \sem{x}\env(\pi_1^0) = v
 \land v > 0 \land 
 \pi_{s_0} = {}^0  \land
 {}^0 \pi_{s_i} {}^0 = {}^0 \xrightarrow{(x > 0)} {}^1 \xrightarrow{x = v - i} {}^0\right\}
 \\ & \cup 
 \left\{ \left< \pi_1^0, {}^0 \xrightarrow{\neg(x > 0)} {}^{\mathsf{aft}\sem{S}} \right> 
 \mid \pi_1^0 \in \mathbb{T^{+}} \land v \in \mathbb{N} \land
  \sem{x}\env(\pi_1^0) = v
 \land v \leq 0 \right\}
\\ & \cup 
 \left\{ \left< \pi_1^0, {}^0 \pi_{s_1} {}^0 \cdots {}^0 \pi_{s_v} {}^0 \xrightarrow{\neg(x > 0)} {}^{\mathsf{aft}\sem{S}}\right>
 \mid \pi_i^0 \in \mathbb{T^{+}} \land v \in \mathbb{N} \land
 \sem{x}\env(\pi_1^0) = v
 \land v > 0  \land
 {}^0 \pi_{s_i} {}^0 = {}^0 \xrightarrow{(x > 0)} {}^1 \xrightarrow{x = v - i} {}^0
 \right\}
 \end{array}
 \]
 %
 \[
 \begin{array}{ll}
  \mathcal{S}^{+}\sem{\ewhile {}^0 (x > 0) {}^1 x = x - 1;} 
  & \triangleq \left\{ \config{\pi_1, \pi_2^{l}} \in \mathcal{S}^{*}\sem{\ewhile {}^0 (x > 0) {}^1 x = x - 1;} \mid l = \mathsf{aft}\sem{S}
  \right\}\\
  & = \Big\{ \left< \pi_1^0, {}^0 \pi_{s_1} {}^0 \cdots {}^0 \pi_{s_v} {}^0 \xrightarrow{\neg(x > 0)} {}^{\mathsf{aft}\sem{S}}\right>
 \mid \pi_i^0 \in \mathbb{T^{+}} \land v \in \mathbb{N} \land
 \sem{x}\env(\pi_1^0) = v
 \land v > 0  
 \\ & \qquad \land
 {}^0 \pi_{s_i} {}^0 = {}^0 \xrightarrow{(x > 0)} {}^1 \xrightarrow{x = v - i} {}^0
 \Big\}
  \\ & \quad \cup 
 \left\{ \left< \pi_1^0, {}^0 \xrightarrow{\neg(x > 0)} {}^{\mathsf{aft}\sem{S}} \right> 
 \mid \pi_1^0 \in \mathbb{T^{+}} \land v \in \mathbb{N} \land
  \sem{x}\env(\pi_1^0) = v
 \land v \leq 0 \right\}
\end{array}
 \]
 %
  if $\forall i \in \mathbb{N} \st \exists v \in \mathbb{N} \st 
  v - i = \infty - i$, then
 \[
 \begin{array}{ll}
  \mathcal{S}^{\infty}\sem{\ewhile {}^0 (x > 0) {}^1 x = x - 1;} 
  & \triangleq \lim(\mathcal{S}^*\sem{\ewhile {}^0 (x > 0) {}^1 x = x - 1;}) 
  \\
  & \triangleq \left\{ \config{\pi_1, \pi_2} \mid 
  \pi_2 \in \mathbb{T}^{\infty} \land \forall n \in \mathbb{N} \st \config{\pi_1, \pi_2[0..n]}\in \mathcal{S}^{*}\sem{\ewhile {}^0 (x > 0) {}^1 x = x - 1;}
  \right\}
  \\
  & = \left\{ \left< \pi_1^0, {}^0 \pi_{s_1} {}^0 \cdots \right>
 \mid \pi_i^0 \in \mathbb{T^{+}} \land
 \sem{x}\env(\pi_1^0) = \infty
 \land
 {}^0 \pi_{s_i} {}^0 = {}^0 \xrightarrow{(x > 0)} {}^1 \xrightarrow{x = \infty - i} {}^0
 \right\}
 \end{array}
 \]
 %
  Since $\not\exists v \in \mathbb{N} \st v = \infty$, 
 \[
   \mathcal{S}^{\infty}
   \sem{\ewhile {}^0 (x > 0) {}^1 x = x - 1;}
   = \emptyset
 \]
 %
 if $\exists v \in \mathbb{N} \st v = \max(\mathbb{N})$, then
  \[
 \begin{array}{ll}
  \mathcal{S}^{\infty}\sem{\ewhile {}^0 (x > 0) {}^1 x = x - 1;}
  &  = \left\{ \left< \pi_1^0, {}^0 \pi_{s_1} {}^0 \cdots \pi_{s_{v}} {}^0 \right>
 \mid \pi_i^0 \in \mathbb{T^{+}} \land
 \sem{x}\env(\pi_1^0) = v
 \land
 {}^0 \pi_{s_i} {}^0 = {}^0 \xrightarrow{(x > 0)} {}^1 \xrightarrow{x = v - i} {}^0
 \right\}
 \end{array}
 \]
 %
 Since $\not\exists v \in \mathbb{N} \st v = \max(\mathbb{N})$, 
 \[
   \mathcal{S}^{\infty}\sem{\ewhile {}^0 (x > 0) {}^1 x = x - 1;}
   = \emptyset
 \]
 %
  \[
 \begin{array}{ll}
  \mathcal{S}^{+\infty}\sem{\ewhile {}^0 (x > 0) {}^1 x = x - 1;} 
 &  \triangleq \mathcal{S}^{+\infty}\sem{\ewhile {}^0 (x > 0) {}^1 x = x - 1;} 
  \cup
  \mathcal{S}^{+\infty}\sem{\ewhile {}^0 (x > 0) {}^1 x = x - 1;}
  \\
   & = \Big\{ \left< \pi_1^0, {}^0 \pi_{s_1} {}^0 \cdots {}^0 \pi_{s_v} {}^0 \xrightarrow{\neg(x > 0)} {}^{\mathsf{aft}\sem{S}}\right>
 \mid \pi_i^0 \in \mathbb{T^{+}} \land v \in \mathbb{N} \land
 \sem{x}\env(\pi_1^0) = v
 \land v > 0  \\
 & \qquad \land
 {}^0 \pi_{s_i} {}^0 = {}^0 \xrightarrow{(x > 0)} {}^1 \xrightarrow{x = v - i} {}^0
 \Big\}
   \\ & \quad \cup 
 \left\{ \left< \pi_1^0, {}^0 \xrightarrow{\neg(x > 0)} {}^{\mathsf{aft}\sem{S}} \right> 
 \mid \pi_1^0 \in \mathbb{T^{+}} \land v \in \mathbb{N} \land
  \sem{x}\env(\pi_1^0) = v
 \land v \leq 0 \right\}
 \end{array}
 \]
 %
 \end{example}
 %
 \begin{example}
 \[
 \begin{array}{ll}
 & \mathcal{S}^{*}\sem{ 
 \epsilon {}^0 x = 1; \ewhile {}^1  (x > 0) {}^2 x = x - 1 ; {}^3 }  \\
 \triangleq & 
 \sem{\epsilon {}^0 x = 1;} 
 \cup
 \left\{ \left< \pi_1{}^0, {}^0\pi_2^1\pi_3^3\right> 
 \left \vert 
 \begin{array}{l}
 \left< \pi_1^0, {}^0\pi_2^1 \right> \in \sem{\epsilon {}^0 x = 1;}
 \\
 \land \left< \pi_1{}^0\pi_2^1, {}^1\pi_3^3\right>  \in 
 \sem{\ewhile {}^1 (x > 0) {}^2 x = x - 1 ;} 
 \end{array}
 \right.
 \right\}
 \\
 \triangleq & 
 \sem{\epsilon}
 \cup
 \left\{ \left< \pi_1{}^0, {}^0 \pi_2 {}^1 \right> 
 \left \vert 
 \begin{array}{l}
 \left< \pi_1{}^0, {}^0 \right> \in \sem{\epsilon}  \land \\
  
 \left< \pi_1{}^0, {}^0 \pi_2{}^1 \right> \in \sem{ {}^0 x = 1;}
 \end{array}
 \right.
 \right\}
 \cup
 \left\{ \left< \pi_1{}^0, {}^0\pi_2^1\pi_3 {}^3\right> 
 \left \vert 
 \begin{array}{l}
 \left< \pi_1{}^0, {}^0\pi_2^1 \right> \in \sem{\epsilon {}^0 x = 1;}\land
 \\
  \left< \pi_1 {}^0\pi_2 {}^1, {}^1 \pi_3 {}^3\right>  \in 
 \sem{\ewhile {}^1  (x > 0) {}^2 x = x - 1 ;} 
 \end{array}
 \right.
 \right\}
 \\
 \triangleq 
 & \left\{ \left< \pi_1^0, ^0\right> \mid \pi_1^0 \in \mathbb{T^{+}} \right\} \\
 & \cup
 \left\{ \left< \pi_1{}^0, {}^0 \xrightarrow{(x = 1) = 1} {}^1\right> 
 \vert 
 \pi_1^0 \in \mathbb{T^{+}}
 \land 
 \sem{1}\env(\pi_1^0) = 1
 \right\} \\
 & \cup
 \left\{ \left< \pi_1{}^0, {}^0\xrightarrow{(x = 1) = 1} {}^1\pi_3^3\right> 
 \left \vert 
 % \begin{array}{l}
 \pi_1^0 \in \mathbb{T^{+}}
 \land
 \left< \pi_1 {}^0\xrightarrow{(x = 1) = 1} {}^1, {}^1\pi_3^3\right>  \in 
 \sem{\ewhile {}^1  (x > 0) {}^2 x = x - 1 ; {}^3} 
 % \end{array}
 \right.
 \right\}
 \\ = & 
 \left\{ \left< \pi_1^0, ^0\right> \mid \pi_1^0 \in \mathbb{T^{+}} \right\} 
 \\ & \cup
 \left\{ \left< \pi_1{}^0, {}^0 \xrightarrow{(x = 1) = 1} {}^1\right> 
 \vert 
 \pi_1^0 \in \mathbb{T^{+}}
 \land 
 \sem{1}\env(\pi_1^0) = 1
 \right\} 
 \\ & \cup 
 \left\{ \left< \pi_1^0, {}^0 \xrightarrow{(x = 1) = 1} {}^1 \xrightarrow{(x > 0)} {}^2 \xrightarrow{(x = x - 1) = 0} {}^1 \right> 
 \left \vert
 \begin{array}{l}
 \pi_i^0 \in \mathbb{T^{+}} \\
 \land 
 \sem{(x > 0)}\env(\pi_1{}^0 \xrightarrow{(x = 1) = 1} {}^1) = \etrue  \\
 \land
 \sem{(x - 1)}\env(\pi_1{}^0 \xrightarrow{(x = 1) = 1} {}^1 \xrightarrow{(x > 0)} {}^2) = 0
 \end{array}
 \right.
 \right\}
 \\ & \cup 
 \left\{ \left< \pi_1^0, {}^0 \xrightarrow{(x = 1) = 1} {}^1 \xrightarrow{(x > 0)} {}^2 \xrightarrow{(x = x - 1) = 0} {}^1 
 \xrightarrow{\neg(x > 0)} {}^3 \right> 
 \left \vert
 \begin{array}{l}
 \pi_i^0 \in \mathbb{T^{+}} \\
 \land 
 \sem{(x > 0)}\env(\pi_1{}^0 \xrightarrow{(x = 1) = 1} {}^1) = \etrue  
 \\ \land
 \sem{(x - 1)}\env(\pi_1{}^0 \xrightarrow{(x = 1) = 1} {}^1 \xrightarrow{(x > 0)} {}^2) = 0 \\
 \land 
 \sem{(x > 0 )}\env(\pi_1{}^0 \xrightarrow{(x = 1) = 1} {}^1 \xrightarrow{(x > 0)} {}^2 \xrightarrow{(x = x - 1) = 0} {}^1) =\efalse
 \end{array}
 \right.
 \right\}
 \\ = & 
 \left\{ \left< \pi_1^0, ^0\right> \mid \pi_1^0 \in \mathbb{T^{+}} \right\} 
  \cup
 \left\{ \left< \pi_1{}^0, {}^0 \xrightarrow{(x = 1) = 1} {}^1\right> 
 \vert 
 \pi_1^0 \in \mathbb{T^{+}}
 \right\} 
 \\ & \cup 
 \left\{ \left< \pi_1^0, {}^0 \xrightarrow{(x = 1) = 1} {}^1 \xrightarrow{(x > 0)} {}^2 \xrightarrow{(x = x - 1) = 0} {}^1 \right> 
 \vert \pi_i^0 \in \mathbb{T^{+}}
 \right\}
 \\ & \cup 
 \left\{ \left< \pi_1^0, {}^0 \xrightarrow{(x = 1) = 1} {}^1 \xrightarrow{(x > 0)} {}^2 \right> 
 \vert \pi_i^0 \in \mathbb{T^{+}}
 \right\}
 \\ & \cup 
 \left\{ \left< \pi_1^0, {}^0 \xrightarrow{(x = 1) = 1} {}^1 \xrightarrow{(x > 0)} {}^2 \xrightarrow{(x = x - 1) = 0} {}^1 
 \xrightarrow{\neg(x > 0)} {}^3 \right> 
 \vert \pi_i^0 \in \mathbb{T^{+}}
 \right\}
 \end{array}
 \]
 %
 \[
 \mathcal{S}^{+}\sem{ 
 \epsilon {}^0 x = 1; \ewhile {}^1  (x > 0) {}^2 x = x - 1 ; {}^3 }  
 = \left\{ \left< \pi_1^0, {}^0 \xrightarrow{(x = 1) = 1} {}^1 \xrightarrow{(x > 0)} {}^2 \xrightarrow{(x = x - 1) = 0} {}^1 
 \xrightarrow{\neg(x > 0)} {}^3 \right> 
 \vert \pi_i^0 \in \mathbb{T^{+}}
 \right\}
 \]
 %
 \[
 \mathcal{S}^{\infty}\sem{ 
 \epsilon {}^0 x = 1; \ewhile {}^1  (x > 0) {}^2 x = x - 1 ; {}^3} = \emptyset
 \]
 %
 \[
 \begin{array}{ll}
 \mathcal{S}^{+\infty}\sem{ 
 \epsilon {}^0 x = 1; \ewhile {}^1  (x > 0) {}^2 x = x - 1 ; {}^3 } 
 & \triangleq \mathcal{S}^{+}\sem{ 
 \epsilon {}^0 x = 1; \ewhile {}^1  (x > 0) {}^2 x = x - 1 ; {}^3} 
 \\ & \cup  
 \mathcal{S}^{\infty}\sem{ 
 \epsilon {}^0 x = 1; \ewhile {}^1  (x > 0) {}^2 x = x - 1 ; {}^3}\\
 & = \left\{ \left< \pi_1^0, {}^0 \xrightarrow{(x = 1) = 1} {}^1 \xrightarrow{(x > 0)} {}^2 \xrightarrow{(x = x - 1) = 0} {}^1 
 \xrightarrow{\neg(x > 0)} {}^3 \right> 
 \vert \pi_i^0 \in \mathbb{T^{+}}
 \right\}
 \end{array}
 \]
 \end{example}
 %
 \clearpage
 \begin{example}[Formal Example for Exclusion of Timing Channel].
 \label{ex:excltiming}
 \\
 $\mathsf{diff}(\omega, \omega')$ (in \cite{cousot2019abstract} Equation~(2)) excludes timing channel,(i.e., $\omega$ is a strict prefix of $\omega'$). There is an example showing this exclusion: 
 \[
 	\ewhile {}^0 (x > 0) {}^1 y = 1;
 \]
 In this example, $y$'s execution times relies on value of $x$. Under the adaptivity scenario, $y$ depends on $x$ (control dependency).
 However, according to value dependency defined in Definition~2 \cite{cousot2019abstract}, we can never derive :
 \[
 	x \rightsquigarrow^{1}_{\ewhile {}^0 (x > 0) {}^1  y = 1;} y
 \]
 %
 \begin{proof}
 By semantics definition, we have:
 %
 \[
 \begin{array}{ll}
 \mathcal{S}^{*} \sem{ \ewhile {}^0 (x > 0) {}^1 y = 1; } 
 & =  \left\{ \left< \pi_1^0, ^0\right> \mid \pi_1^0 \in \mathbb{T^{+}} \right\}
 \\ &  \cup 
 \left\{ \left< \pi_1^0, {}^0 \pi_2 {}^0 \pi_2 {}^0\cdots \right>
 \mid \pi_i^0 \in \mathbb{T^{+}} \land v \in \mathbb{N} \land
 \sem{x}\env(\pi_1^0) = v
 \land v > 0  \land
 {}^0 \pi_2 {}^0 = {}^0 \xrightarrow{(x > 0)} {}^1 \xrightarrow{y = 1} {}^0
 \right\}
 \\ &  \cup 
 \Big\{ \left< \pi_1^0, {}^0 \pi_0 {}^0 \pi_2 {}^0 \cdots {}^0 \pi_2 {}^0 \xrightarrow{(x > 0)} {}^1 \right>
 \mid \pi_i^0 \in \mathbb{T^{+}} \land v \in \mathbb{N} \land
 \sem{x}\env(\pi_1^0) = v
 \land v > 0 \land 
 \pi_0 = {}^0  
 \\ & \qquad \land
 {}^0 \pi_2 {}^0 = {}^0 \xrightarrow{(x > 0)} {}^1 \xrightarrow{y = 1} {}^0
 \Big\}
 \\ & \cup 
 \left\{ \left< \pi_1^0, {}^0 \xrightarrow{\neg(x > 0)} {}^{\mathsf{aft}\sem{S}} \right> 
 \mid \pi_1^0 \in \mathbb{T^{+}} \land v \in \mathbb{N} \land
  \sem{x}\env(\pi_1^0) = v
 \land v \leq 0 \right\}
 \end{array}
 \]
 \begin{equation}
 \label{eq:sem_timingdep}
 \begin{array}{ll}
\mathcal{S}^{+\infty} \sem{ \ewhile {}^0 (x > 0) {}^1 y = 1; } 
& =  
 \left\{ \left< \pi_1^0, {}^0 \pi_2 {}^0 \pi_2 {}^0\cdots \right>
 \mid \pi_i^0 \in \mathbb{T^{+}} \land v \in \mathbb{N} \land
 \sem{x}\env(\pi_1^0) = v
 \land v > 0  \land
 {}^0 \pi_2 {}^0 = {}^0 \xrightarrow{(x > 0)} {}^1 \xrightarrow{y = 1} {}^0
 \right\}
 \\ & \quad \cup 
 \left\{ \left< \pi_1^0, {}^0 \xrightarrow{\neg(x > 0)} {}^{\mathsf{aft}\sem{S}} \right> 
 \mid \pi_1^0 \in \mathbb{T^{+}} \land v \in \mathbb{N} \land
  \sem{x}\env(\pi_1^0) = v
 \land v \leq 0 \right\}
 \end{array} 
 \end{equation}
 %
 %
 %
 Let $\pi_1, \pi_1' \in \mathbb{T^{+}}$ be arbitrary traces s.t. 
 %
 $$\forall z \in \mathbb{V}\setminus \{x\}. ~ \env(\pi_1)(z) = \env(\pi_1')(z) $$ 
 %
 Without loss of generalization, let $\env(\pi_1)(y) = \env(\pi_1')(y) = 0$
 %
 Let $v = \env(\pi_1)(x) $, $v' = \env(\pi'_1)(x')$, picking arbitrary $\pi_2, \pi_2'$ s.t.:
 \[
 	\left< \pi_1, \pi_2 \right>,  \left< \pi'_1, \pi'_2 \right> 
  \in \mathcal{S}^{+\infty}\sem{\ewhile {}^0 (x > 0) {}^1 y = 1; }
 \]
 %
 There are 3 cases:
 \caseL{$v, v' > 0:$}
 %
 Then we know:
 \[
 \pi_2 = {}^0 \pi' {}^0 \pi' {}^0\cdots 
\]
%
\[ 
 \pi_2' = {}^0 \pi' {}^0 \pi' {}^0\cdots 
 \]
 %
 where ${}^0 \pi' {}^0 = {}^0 \xrightarrow{(x > 0)} {}^1 \xrightarrow{y = 1} {}^0$.
 %
 \\
 By Definition of $\mathsf{seqval}$, we have:
 \[
  \mathsf{seqval}\sem{y}{}^1(\pi_1, \pi_2 ) =  0 \cdot \underbrace{ \cdots 1 \cdots}_{\infty}
 \]
 %
 \[
  \mathsf{seqval}\sem{y}{}^1(\pi_1', \pi_2' ) =  0 \cdot \underbrace{\cdots 1  \cdots}_{\infty}
 \]
 %
  $\forall \omega_0, \omega_1', \omega_1, u, u' \st 
  0 \cdot \underbrace{0 \cdots 1}_{0 \leq v} = \omega \cdot u \cdot \omega_1 
  \land 0 \cdot \underbrace{0 \cdots 1}_{0 \leq v} = \omega \cdot u' \cdot \omega_1'$ we have:
 %
 \[
  u = u'
 \]
 %
 By $\mathsf{diff}(\omega, \omega')$ (in \cite{cousot2019abstract} Equation~(2) ), we have:
 %
 \[
  \neg(\mathsf{diff}(\mathsf{seqval}\sem{y}{}^1(\pi_1, \pi_2 ), \mathsf{seqval}\sem{y}{}^1(\pi_1', \pi_2' )))
 \]
 \caseL{$v > 0, v' \leq 0$ ($v \leq 0, v' > 0$ will be the symmetric case proved in the same way)}
 Then we know:
  \[
  \pi_2 = {}^0 \pi' {}^0 \pi' {}^0 \cdots 
  \]
  \[
  \pi_2' = {}^0 \xrightarrow{\neg(x > 0)} {}^{\mathsf{aft}\sem{S}}
  \]
 %
 where ${}^0 \pi' {}^0 = {}^0 \xrightarrow{(x > 0)} {}^1 \xrightarrow{y = 1} {}^0$.
 %
 By Definition of $\mathsf{seqval}$, we have:
 \[
  \mathsf{seqval}\sem{y}{}^1(\pi_1, \pi_2 ) = 0 \cdot \underbrace{1 \cdots}_{\infty}
 \]
 %
 \[
  \mathsf{seqval}\sem{y}{}^1(\pi'_1, \pi_2' ) = \epsilon
 \]
 %
 Since $\forall \omega_0, \omega_1', \omega_1, u\st \not\exists u' \st 
  0 \cdot \underbrace{0 \cdots 1}_{\infty} = \omega \cdot u \cdot \omega_1 
  \land \epsilon = \omega \cdot u' \cdot \omega_1'$,
 we have by definition $\mathsf{diff}(\omega, \omega')$ (in \cite{cousot2019abstract} Equation~(2) ), we have:
 %
 \[
  \neg(\mathsf{diff}(\mathsf{seqval}\sem{y}{}^1(\pi_1, \pi_2 ), \mathsf{seqval}\sem{y}{}^1(\pi_1', \pi_2' )))
 \]
 \caseL{$v, v' \leq 0$}
 %
 Then we know:
 \[
 \pi_2 = {}^0 \pi' {}^0 \pi' {}^0\cdots 
 \land 
 \pi_2' = {}^0 \xrightarrow{\neg(x > 0)} {}^{\mathsf{aft}\sem{S}}
 \]
 %
 where ${}^0 \pi' {}^0 = {}^0 \xrightarrow{(x > 0)} {}^1 \xrightarrow{y = 1} {}^0$.
 %
 By Definition of $\mathsf{seqval}$, we have:
 \[
  \mathsf{seqval}\sem{y}{}^1(\pi_1, \pi_2 ) = \epsilon
 \]
 %
 \[
  \mathsf{seqval}\sem{y}{}^1(\pi_1', \pi_2' ) = \epsilon
 \]
 %
  $\not \exists \omega_0, \omega_1', \omega_1, u, u' \st 
  \epsilon = \omega \cdot u \cdot \omega_1 
  \land 
  \epsilon = \omega \cdot u; \cdot \omega_1'$
 %
 By $\mathsf{diff}(\omega, \omega')$ (in \cite{cousot2019abstract} Equation~(2) ), we have:
 %
 \[
  \neg(\mathsf{diff}(\mathsf{seqval}\sem{y}{}^1(\pi_1, \pi_2 ), \mathsf{seqval}\sem{y}{}^1(\pi_1', \pi_2' )))
 \]
 In all three cases, we have:
 \[
   \neg(\mathsf{diff}(\mathsf{seqval}\sem{y}{}^1(\pi_1, \pi_2 ), \mathsf{seqval}\sem{y}{}^1(\pi_1', \pi_2' )))
 \]
 Then we have the conclusion as follows:
 \[
 \begin{array}{l}
 	\forall \left< \pi_1, \pi_2 \right>,  \left< \pi_1', \pi'_2 \right> \in \mathcal{S}^{+\infty} \sem{\ewhile {}^0 (x > 0) {}^1 y = 1;} \st
 	\Big(
 	\forall z \in \mathbb{V}\setminus \{x\} \st \env(\pi_1)(z) = \env(\pi_1') \st \\
 	\land \neg(\mathsf{diff}(\mathsf{seqval}\sem{y}{}^1(\pi_1, \pi_2), \mathsf{seqval}\sem{y}{}^1(\pi_1', \pi_2' )))\Big)
 \end{array}
 \] 
 \\
 %
 By Definition~2 (in \cite{cousot2019abstract}), 
 \[
 	\mathcal{S}^{+\infty}\sem{\ewhile {}^0 (x > 0) {}^1 y = 1;} 
 \notin \mathcal{D}^1(z, y)
 \]
 %
 By Definition~(4) (in \cite{cousot2019abstract}), we cannot derive:
 \[
 	x \rightsquigarrow^{1}_{\ewhile {}^0 (x > 0) {}^1 y = 1;} y
 \]
 %
 %
 \end{proof}
 \end{example}
 %
 \clearpage
 \begin{example}[Approach-1 of Including Timing Channel].
 \label{ex:overapp}
 \\
 If $\mathsf{diff}(\omega, \omega')$ (in \cite{cousot2019abstract} Equation~(2)) simply includes timing channel,(i.e., $\omega$ is a strict prefix of $\omega'$) as follows:
 \[
 	\mathsf{diff}(\omega, \omega') \triangleq \exists \omega_0, \omega_1, \omega_1', v, v' 
 	\st \bigvee \left\{
 	\begin{array}{lr}
 	(\omega = \omega_0 \cdot v \omega_1
 		\land \omega' = \omega_0 \cdot v' \omega_1' \land v \neq v') & \mbox{original definition} \\
 	(\omega = \omega' \cdot v \cdot \omega_1) & \mbox{including timing channel} \\
 	\end{array}
 	\right\}
 \] 
 then by Definition~2 (in \cite{cousot2019abstract}), the value dependency relation between $x$ and $y$ in the same example as \ref{eq:sem_timingdep} can be derived:
 \[
 	\ewhile {}^2 (x > 0) {}^3 y = 1; 
 \]
  \[
 	x \rightsquigarrow^{2}_{\ewhile {}^2 (x > 0) {}^3 y = 1;} y
 \]
 %
 \begin{proof}
 By semantics definition, we have:
 %
 \begin{equation}
 \label{eq:sem_timingoverapp}
 \begin{array}{ll}
   \mathcal{S}^{+\infty}\sem{ \ewhile {}^2 (x > 0) {}^3 y = 1; } 
 & \triangleq  
 \left\{ \left< \pi_1{}^2, {}^2 \pi_2 {}^2 \pi_2 {}^2\cdots \right>
 \mid \pi_i^0 \in \mathbb{T^{+}} \land v \in \mathbb{N} \land
 \sem{x}\env(\pi_1) = v
 \land v > 0  \land
 \pi_2 = {}^2 \xrightarrow{(x > 0)} {}^1 \xrightarrow{y = 1} {}^2
 \right\}
 \\ & \quad \cup 
 \left\{ \left< \pi_1, {}^2 \xrightarrow{\neg(x > 0)} {}^{\mathsf{aft}\sem{S}} \right> 
 \mid \pi_1 \in \mathbb{T^{+}} \land v \in \mathbb{N} \land
  \sem{x}\env(\pi_1) = v
 \land v \leq 0 \right\}
 \end{array}
 \end{equation}
 %
 %
 Pick $\pi_1 =  {}^1 \xrightarrow{x = 1} {}^2$, 
 $\pi_1' =  {}^1 \xrightarrow{x = 0} {}^2$, we have
 \[
 	\left< \pi_1, {}^2 \pi' {}^2 \pi' {}^2 \cdots \right> \in \sem{\ewhile {}^2 (x > 0) {}^3 y = 1;}
 \]
 %
 \[
 	\left< \pi_1', {}^2 \xrightarrow{\neg(x > 0)} {}^{\mathsf{aft}\sem{S}}\right> \in \sem{\ewhile {}^2 (x > 0) {}^3 y = 1; }
 \]
 %
 where $\pi' = {}^2 \xrightarrow{(x > 0)} {}^3 \xrightarrow{y = 1} {}^2$
 %
By Definition of $\mathsf{seqval}$, we have:
 \[
  \mathsf{seqval}\sem{y}{}^2(\pi_1, \pi_2 ) = 0 \cdot \underbrace{1 \cdots}_{\infty}
 \]
 %
 \[
  \mathsf{seqval}\sem{y}{}^2(\pi'_1, \pi_2' ) = \epsilon
 \]
 %
 Since $\underbrace{1 \cdots}_{\infty} = \epsilon \cdot 0 \cdot \underbrace{1 \cdots}_{\infty}$,
 we have by modified definition $\mathsf{diff}(\omega, \omega')$ (above), we have:
 %
 \[
  (\mathsf{diff}(\mathsf{seqval}\sem{y}{}^1(\pi_1, \pi_2 ), \mathsf{seqval}\sem{y}{}^1(\pi_1', \pi_2' )))
 \]
 %
  By Definition~2 (in \cite{cousot2019abstract}), 
 \[
  \mathcal{S}^{+\infty}\sem{\ewhile {}^2 (x > 0) {}^3 y = 1;} 
 \notin \mathcal{D}^2(x, y)
 \]
 %
 By Definition~(4) (in \cite{cousot2019abstract}), we cannot derive:
 \[
  x \rightsquigarrow^{2}_{\ewhile {}^2 (x > 0) {}^3 y = 1;} y
 \]

 \end{proof}
 \end{example}
 %
 % \clearpage
 % \begin{example}[Approach-2 of Including Timing Channel]
 % Modifying the Definition~2 (in \cite{cousot2019abstract}) as follows:
 % \begin{defn}[Modified Data Dependency].
 % \label{defn:mdfy_dep}
 % \[
 % 	\begin{array}{lll}
 % 	\mathcal{D}^l(x, y) & \triangleq &
 % 	\Big\{ 
 % 	\Pi \in (\mathbb{T}^{+} \times \mathbb{T}^{+\infty})
 % 	\exists \config{\pi_1, \pi_2}, \config{\pi_1', \pi_2'} \in \Pi \st \\
 % 	&& \quad \big(
 % 	\forall z \in \mathbb{V}\setminus \{x\} \st \env(\pi_1)(z) = \env(\pi_1') \st \\
 % 	&& \quad  \quad \land \neg(\mathsf{diff}(\mathsf{seqval}\sem{y}{}^1(\pi_1, \pi_2 ), \mathsf{seqval}\sem{y}{}^1(\pi'_1, \pi_2')))
 % 	\big) \Big\} \\
 % 	& \cup & \Big\{ \Pi \in (\mathbb{T}^{+} \times \mathbb{T}^{+\infty})
 % 	\exists \config{\pi_1, \pi_2}, \config{\pi_1', \pi_2'} \in \Pi \st \forall \config{\pi_1', \pi_2''} \in \Pi\\
 % 	&& \quad \big(
 % 	\forall z \in \mathbb{V}\setminus \{x\} \st \env(\pi_1)(z) = \env(\pi_1') \st \\
 % 	&& \quad  \quad  \land |\mathsf{seqval}\sem{y}{}^1(\pi_1', \pi_2'')| \leq |\mathsf{seqval}\sem{y}{}^1(\pi_1', \pi_2')| <  
 % 	|\mathsf{seqval}\sem{y}{}^1(\pi_1, \pi_2)|\big) \Big\}
 % 	\end{array}
 % \]
 % \end{defn}
 % This definition is capable to include the timing channel(control dependency) in Example~\ref{ex:excltiming},
 % as well as exclude the over approximation in Example~\ref{ex:overapp}.
 % %
 % \begin{proof}
 % \caseL{Including the Example~\ref{ex:excltiming}}
 % By Example~\ref{ex:excltiming}, we have its semantics in Equation~\ref{eq:sem_timingdep}.
 % %
 % %
 % Let $\pi_1^0, \pi_1'^0 \in \mathbb{T^{+}}$ be arbitrary traces s.t. 
 % %
 % $$\forall z \in \mathbb{V}\setminus \{x\}. ~ \env(\pi_1^0)(z) = \env(\pi_1'^0) $$ 
 % %
 % Let $v = \env(\pi_1^0)(x)$, $v' = \env(\pi_1'^0)(x')$, without lose of generalization, let $0 \leq v' < v$.
 % \\
 % Let 
 % $t_i = {}^2 \xrightarrow{(x = x - 1) = v - i } {}^3 \xrightarrow{(y = 1) = 1} {}^0 \cdots  {}^0$, for $i = 1, \cdots, v$
 % %
 % $\pi_2 = {}^0 \xrightarrow{(x > 0)} {}^2 t_1 {}^0 \cdots   {}^2 t_v {}^0 \xrightarrow{\neg(x > 0)} {}^l $,
 % %
 %  By Equation~\ref{eq:sem_timingdep}, we know:
 % \[
 % 	\left< \pi_1^0, \pi_2 \right> \in \sem{\ewhile {}^0 (x > 0) \{{}^2 x = x - 1; {}^3 y = 1;\} }
 % \]
 % %
 % Let 
 % $t_i' = {}^2 \xrightarrow{(x = x - 1) = v' - i } {}^3 \xrightarrow{(y = 1) = 1} {}^0 \cdots  {}^0$, for $i = 1, \cdots, v'$
 % %
 % $\pi_2' = {}^0 \xrightarrow{(x > 0)} {}^2 t'_1 {}^0 \cdots  {}^2 t'_{v'} {}^0 \xrightarrow{\neg(x > 0)} {}^l $,
 % %
 %  By Equation~\ref{eq:sem_timingdep}, we know:
 % \[
 % 	\left< \pi_1'^0, \pi'_2 \right> \in \sem{\ewhile {}^0 (x > 0) \{{}^2 x = x - 1; {}^3 y = 1;\} }
 % \]
 % %
 % \\
 % By Definition of $\mathsf{seqval}$, we have:
 % \[
 % 	|\mathsf{seqval}\sem{y}{}^0(\pi_1^0, \pi_2 )| = |\underbrace{0 \cdots 1}_{0 \leq v}| = v + 1
 % \]
 % %
 % \[
 % 	|\mathsf{seqval}\sem{y}{}^0(\pi_1^0, \pi_2' )| = |\underbrace{0 \cdots 1}_{0 \leq v'}| = v' + 1
 % \]
 % %
 % Since, $v' < v $, we have: 
 % \[
 % 	|\mathsf{seqval}\sem{y}{}^0(\pi_1^0, \pi_2' )| < |\mathsf{seqval}\sem{y}{}^0(\pi_1^0, \pi_2 )|
 % \]
 % %
 % Let $\Pi_2''$ defined as follows:
 % \[
 % 	\Pi''_2 \triangleq \{
 % 	\left< \pi_1'^0, \pi''_2 \right> \vert
 % 	\pi''_2 =  {}^0 \xrightarrow{(x > 0)} {}^2 t'_1 {}^0 \cdots  {}^2 t'_{j} {}^0, \forall j < v'\} 
 % \]
 % %
 % By Equation~\ref{eq:sem_timingdep}, we know:
 % %
 % \[
 % 		\Pi''_2 \subseteq \sem{\ewhile {}^0 (x > 0) \{{}^2 x = x - 1; {}^3 y = 1;\} }
 % 		\land
 % 		\forall \left< \pi_1', \pi''_2 \right> \in \sem{\ewhile {}^0 (x > 0) \{{}^2 x = x - 1; {}^3 y = 1;\} } 
 % 		\st \left< \pi_1', \pi''_2 \right> \in  \Pi''_2
 % \]
 % %

 % %
 % %
 % Then for arbitrary $\left< \pi_1', \pi''_2 \right> \in \sem{\ewhile {}^0 (x > 0) \{{}^2 x = x - 1; {}^3 y = 1;\} }$, we know:
 % \[
 % 	\exists \st \pi''_2 =  {}^0 \xrightarrow{(x > 0)} {}^2 t'_1 {}^0 \cdots  {}^2 t'_{j} {}^0 \land j \leq v'
 % \]
 % %
 % \[
 % 	|\mathsf{seqval}\sem{y}{}^0(\pi_1^0, \pi_2'' )| = |\underbrace{0 \cdots 1}_{0 \leq j}| = j \leq v'
 % \]
 % %
 % Then we have
 % \[
 % \begin{array}{l}
 % 	\forall \left< \pi_1'^0, \pi''_2 \right> \in \mathcal{S}^{+\infty} \sem{\ewhile {}^2 (x > 0) {}^3 y = 1;} \st
 % 	\Big(
 % 	|\mathsf{seqval}\sem{y}{}^0(\pi_1'^0, \pi_2'' )| \leq v' < v))\Big)
 % \end{array}
 % \] 
 % %
 % i.e.,
 % \[
 % 	\begin{array}{l}
 % 	\exists \config{\pi_1, \pi_2}, \config{\pi_1', \pi_2'} \in \mathcal{S}^{+\infty}\sem{\ewhile {}^0 (x > 0) \{{}^2 x = x - 1; {}^3 y = 1;} \\
 % 	\quad \st \forall \config{\pi_1', \pi_2''} \in \mathcal{S}^{+\infty}\sem{\ewhile {}^0 (x > 0) \{{}^2 x = x - 1; {}^3 y = 1;} \\
 % 	\quad \big(
 % 	\forall z \in \mathbb{V}\setminus \{x\} \st \env(\pi_1)(z) = \env(\pi_1') \st \\
 % 	\quad  \quad  \land |\mathsf{seqval}\sem{y}{}^0(\pi_1', \pi_2'')| 
 % 	\leq |\mathsf{seqval}\sem{y}{}^0(\pi_1', \pi_2')| <  
 % 	|\mathsf{seqval}\sem{y}{}^0(\pi_1, \pi_2)|\big) 	
 % 	\end{array}
 % \]
 % \\
 % %
 % By modified data dependency in Definition~\ref{defn:mdfy_dep} from Definition~2 (in \cite{cousot2019abstract}), we have:
 % \[
 % 	\mathcal{S}^{+\infty}\sem{\ewhile {}^0 (x > 0) \{{}^2 x = x - 1; {}^3 y = 1;} 
 % 	\in \mathcal{D}^0(x, y)
 % \]
 % %
 % By Definition~(4) (in \cite{cousot2019abstract}), we have:
 % \[
 % 	x \rightsquigarrow^{1}_{\ewhile {}^0 (x > 0) \{{}^2 x = x - 1; {}^3 y = 1;\}} y
 % \]
 % %
 % %
 % %
 % \end{proof}
 % \end{example}